ott_coq/destination_calculus_proofs.v
@@ -40,10 +40,10 @@ Proof.
   eapply Permutation.pre_inverse.
 Qed.
 
-Lemma ValidOnlyHvarShiftEquiv: forall (G : ctx) (H : hvars) (h' : hvar), ctx_ValidOnly G <-> ctx_ValidOnly (G ᴳ[ H⩲h' ]).
+Lemma ValidOnlyHvarShiftEquiv: forall (G : ctx) (H : hvars) (h' : hvar), ValidOnly G <-> ValidOnly (G ᴳ[ H⩲h' ]).
 Proof.
-  intros *. unfold ctx_ValidOnly, ctx_hvar_shift.
-  rewrite map_propagate_both with (Q := fun x b => mode_IsValid (binding_mode b)).
+  intros *. unfold ValidOnly, ctx_hvar_shift.
+  rewrite map_propagate_both with (Q := fun x b => IsValid (binding_mode b)).
   2:{ intros [xx|xh] **. all: cbn.
       all: reflexivity. }
   apply precomp_propagate_both. intros x2.
@@ -51,10 +51,10 @@ Proof.
 Qed.
 Hint Rewrite <- ValidOnlyHvarShiftEquiv : propagate_down.
 
-Lemma DestOnlyHvarShiftEquiv: forall (G : ctx) (H : hvars) (h' : hvar), ctx_DestOnly G <-> ctx_DestOnly (G ᴳ[ H⩲h' ]).
+Lemma DestOnlyHvarShiftEquiv: forall (G : ctx) (H : hvars) (h' : hvar), DestOnly G <-> DestOnly (G ᴳ[ H⩲h' ]).
 Proof.
-  intros *. unfold ctx_DestOnly, ctx_hvar_shift.
-  rewrite map_propagate_both with (Q := fun x b => binding_IsDest _ b).
+  intros *. unfold DestOnly, ctx_hvar_shift.
+  rewrite map_propagate_both with (Q := fun x b => IsDest _ b).
   2:{ intros [xx|xh] **. all: cbn.
       all: reflexivity. }
   apply precomp_propagate_both. intros x2.
@@ -62,10 +62,10 @@ Proof.
 Qed.
 Hint Rewrite <- DestOnlyHvarShiftEquiv : propagate_down.
 
-Lemma LinNuOnlyHvarShiftEquiv : forall (G : ctx) (H : hvars) (h' : hvar), ctx_LinNuOnly G <-> ctx_LinNuOnly (G ᴳ[ H⩲h' ]).
+Lemma LinNuOnlyHvarShiftEquiv : forall (G : ctx) (H : hvars) (h' : hvar), LinNuOnly G <-> LinNuOnly (G ᴳ[ H⩲h' ]).
 Proof.
-  intros *. unfold ctx_LinNuOnly, ctx_hvar_shift.
-  rewrite map_propagate_both with (Q := fun x b => mode_IsLinNu (binding_mode b)).
+  intros *. unfold LinNuOnly, ctx_hvar_shift.
+  rewrite map_propagate_both with (Q := fun x b => IsLinNu (binding_mode b)).
   2:{ intros [xx|xh] **. all: cbn.
       all: reflexivity. }
   apply precomp_propagate_both. intros x2.
@@ -73,10 +73,10 @@ Proof.
 Qed.
 Hint Rewrite <- LinNuOnlyHvarShiftEquiv : propagate_down.
 
-Lemma LinOnlyHvarShiftEquiv : forall (G : ctx) (H : hvars) (h' : hvar), ctx_LinOnly G <-> ctx_LinOnly (G ᴳ[ H⩲h' ]).
+Lemma LinOnlyHvarShiftEquiv : forall (G : ctx) (H : hvars) (h' : hvar), LinOnly G <-> LinOnly (G ᴳ[ H⩲h' ]).
 Proof.
-  intros *. unfold ctx_LinOnly, ctx_hvar_shift.
-  rewrite map_propagate_both with (Q := fun x b => mode_IsLin (binding_mode b)).
+  intros *. unfold LinOnly, ctx_hvar_shift.
+  rewrite map_propagate_both with (Q := fun x b => IsLin (binding_mode b)).
   2:{ intros [xx|xh] **. all: cbn.
       all: reflexivity. }
   apply precomp_propagate_both. intros x2.
@@ -84,10 +84,10 @@ Proof.
 Qed.
 Hint Rewrite <- LinOnlyHvarShiftEquiv : propagate_down.
 
-Lemma FinAgeOnlyHvarShiftEquiv : forall (G : ctx) (H : hvars) (h' : hvar), ctx_FinAgeOnly G <-> ctx_FinAgeOnly (G ᴳ[ H⩲h' ]).
+Lemma FinAgeOnlyHvarShiftEquiv : forall (G : ctx) (H : hvars) (h' : hvar), FinAgeOnly G <-> FinAgeOnly (G ᴳ[ H⩲h' ]).
 Proof.
-  intros *. unfold ctx_FinAgeOnly, ctx_hvar_shift.
-  rewrite map_propagate_both with (Q := fun x b => mode_IsFinAge (binding_mode b)).
+  intros *. unfold FinAgeOnly, ctx_hvar_shift.
+  rewrite map_propagate_both with (Q := fun x b => IsFinAge (binding_mode b)).
   2:{ intros [xx|xh] **. all: cbn.
       all: reflexivity. }
   apply precomp_propagate_both. intros x2.
@@ -113,7 +113,7 @@ Proof. Admitted.
 (* TODO: add to canonalize? *)
 
 (* TODO: not true, requires h' to be bigger than the max of H' as well, I believe. *)
-Lemma hvars_max_hvars_Disjoint : forall (H H' : hvars) (h' : hvar), maxᴴ(H) < h' -> H ## (H' ᴴ⩲ h').
+Lemma hvars_max_HDisjoint : forall (H H' : hvars) (h' : hvar), maxᴴ(H) < h' -> H ## (H' ᴴ⩲ h').
 Proof. Admitted.
 
 Lemma hvarsFullShiftEq : forall (G : ctx) (h' : hvar), hvarsᴳ(G ᴳ[ hvarsᴳ( G ) ⩲ h' ]) = hvarsᴳ(G) ᴴ⩲ h'.
@@ -171,12 +171,12 @@ Admitted.
 
 (* ========================================================================= *)
 
-Lemma ValidOnlyUnionBackward : forall (G1 G2 : ctx), ctx_ValidOnly (G1 ᴳ+ G2) -> ctx_ValidOnly G1 /\ ctx_ValidOnly G2.
+Lemma ValidOnlyUnionBackward : forall (G1 G2 : ctx), ValidOnly (G1 ᴳ+ G2) -> ValidOnly G1 /\ ValidOnly G2.
 Proof.
-  assert (forall m1 m2, mode_IsValid (mode_plus m1 m2) -> mode_IsValid m1 /\ mode_IsValid m2) as h_mode_plus.
+  assert (forall m1 m2, IsValid (mode_plus m1 m2) -> IsValid m1 /\ IsValid m2) as h_mode_plus.
   { intros [[p1 a1]|] [[p2 a2]|]. all: cbn.
     all: sfirstorder. }
-  unfold ctx_ValidOnly, ctx_union in *. intros *.
+  unfold ValidOnly, ctx_union in *. intros *.
   eapply (merge_with_propagate_backward).
   intros [xx|xh] [] []. all: cbn.
   all: let rec t := solve
@@ -189,35 +189,35 @@ Proof.
        in t.
 Qed.
 
-Lemma ValidOnlyUnionBackward' : forall (G1 G2 : ctx), Basics.impl (ctx_ValidOnly (G1 ᴳ+ G2)) (ctx_ValidOnly G1 /\ ctx_ValidOnly G2).
+Lemma ValidOnlyUnionBackward' : forall (G1 G2 : ctx), Basics.impl (ValidOnly (G1 ᴳ+ G2)) (ValidOnly G1 /\ ValidOnly G2).
 Proof.
   exact ValidOnlyUnionBackward.
 Qed.
 Hint Rewrite ValidOnlyUnionBackward' : propagate_down.
 
-Lemma ValidOnlyUnionForward : forall (G1 G2 : ctx), ctx_ValidOnly G1 -> ctx_ValidOnly G2 -> G1 # G2 -> ctx_ValidOnly (G1 ᴳ+ G2).
+Lemma ValidOnlyUnionForward : forall (G1 G2 : ctx), ValidOnly G1 -> ValidOnly G2 -> G1 # G2 -> ValidOnly (G1 ᴳ+ G2).
 Proof.
   (* Note: merge_with_propagate_forward doesn't apply to this. Which is why the
      hypothesis `G1 # G2` is needed. *)
-  intros * valid_G1 valid_G2 disjoint_G1G2. unfold ctx_ValidOnly in *.
+  intros * valid_G1 valid_G2 disjoint_G1G2. unfold ValidOnly in *.
   intros n b h. unfold ctx_union in *.
   destruct (In_dec n G1) as [[b1 h_inG1]|h_ninG1]; destruct (In_dec n G2) as [[b2 h_inG2]|h_ninG2]. all: rewrite ?nIn_iff_nMapsTo in *.
-  - sfirstorder unfold: ctx_Disjoint.
+  - sfirstorder unfold: Disjoint.
   - hauto lq: on use: merge_with_Some_None_eq.
   - hauto lq: on use: merge_with_None_Some_eq.
   - hauto lq: on use: merge_with_None_None_eq.
 Qed.
 
-Lemma ValidOnlyUnionForward' : forall (G1 G2 : ctx), Basics.impl (ctx_ValidOnly G1 /\ ctx_ValidOnly G2 /\ G1 # G2) (ctx_ValidOnly (G1 ᴳ+ G2)).
+Lemma ValidOnlyUnionForward' : forall (G1 G2 : ctx), Basics.impl (ValidOnly G1 /\ ValidOnly G2 /\ G1 # G2) (ValidOnly (G1 ᴳ+ G2)).
 Proof.
   intros *. unfold Basics.impl.
   hauto lq: on use: ValidOnlyUnionForward.
 Qed.
 Hint Rewrite <- ValidOnlyUnionForward' : suffices.
 
-Lemma ValidOnlySingletonVar : forall x m T, ctx_ValidOnly ᴳ{ x : m ‗ T} <-> mode_IsValid m.
+Lemma ValidOnlySingletonVar : forall x m T, ValidOnly ᴳ{ x : m ‗ T} <-> IsValid m.
 Proof.
-  intros *. unfold ctx_ValidOnly.
+  intros *. unfold ValidOnly.
   split.
   - intros h.
     specialize (h (ˣ x) (ₓ m ‗ T)). cbn in h.
@@ -231,7 +231,7 @@ Proof.
 Qed.
 Hint Rewrite ValidOnlySingletonVar : propagate_down.
 
-Lemma ValidOnlyStimesBackward : forall (m : mode) (G : ctx), ctx_ValidOnly (m ᴳ· G) -> ctx_ValidOnly G.
+Lemma ValidOnlyStimesBackward : forall (m : mode) (G : ctx), ValidOnly (m ᴳ· G) -> ValidOnly G.
 Proof.
   intros *.
   intros validmG.
@@ -240,62 +240,62 @@ Proof.
       | ʰ _ => binding_stimes_dh m
       end)
     as mf.
-  unfold ctx_ValidOnly in *. intros n binding mapstoG. specialize (validmG n (mf n binding)).
+  unfold ValidOnly in *. intros n binding mapstoG. specialize (validmG n (mf n binding)).
   assert ((m ᴳ· G) n = Some (mf n binding)).
     { eapply map_MapsTo_iff. exists binding. split. tauto. tauto. }
   specialize (validmG H).
   destruct n, binding; cbn in validmG; try rename n into m0; cbn; destruct m0; try constructor; unfold mode_times in validmG; destruct m in validmG; cbn in validmG; try destruct p as (_, _) in validmG; tauto.
 Qed.
 
-Lemma ValidOnlyStimesBackward' : forall (m : mode) (G : ctx), Basics.impl (ctx_ValidOnly (m ᴳ· G)) (ctx_ValidOnly G).
+Lemma ValidOnlyStimesBackward' : forall (m : mode) (G : ctx), Basics.impl (ValidOnly (m ᴳ· G)) (ValidOnly G).
 Proof.
   exact ValidOnlyStimesBackward.
 Qed.
 Hint Rewrite ValidOnlyStimesBackward' : propagate_down.
 
-Lemma TimesIsValidEquiv : forall (m1 m2 : mode), mode_IsValid (m1 · m2) <-> mode_IsValid m1 /\ mode_IsValid m2.
+Lemma TimesIsValidEquiv : forall (m1 m2 : mode), IsValid (m1 · m2) <-> IsValid m1 /\ IsValid m2.
 Proof.
   intros [[p1 a1]|] [[p2 a2]|]. all: cbn.
   all: sfirstorder.
 Qed.
 Hint Rewrite TimesIsValidEquiv : propagate_down.
 
-Lemma ValidOnlyStimesForward : forall (m : mode) (G : ctx), ctx_ValidOnly G /\ mode_IsValid m -> ctx_ValidOnly (m ᴳ· G).
+Lemma ValidOnlyStimesForward : forall (m : mode) (G : ctx), ValidOnly G /\ IsValid m -> ValidOnly (m ᴳ· G).
 Proof.
-  intros * [validG validm]. unfold ctx_ValidOnly, ctx_stimes in *.
+  intros * [validG validm]. unfold ValidOnly, ctx_stimes in *.
   apply map_propagate_forward'.
   - eauto.
   - intros [xx|xh] []. all: cbn.
     all: sfirstorder use: TimesIsValidEquiv.
 Qed.
 
-Lemma ValidOnlyStimesForward' : forall (m : mode) (G : ctx), Basics.impl (ctx_ValidOnly G /\ mode_IsValid m) (ctx_ValidOnly (m ᴳ· G)).
+Lemma ValidOnlyStimesForward' : forall (m : mode) (G : ctx), Basics.impl (ValidOnly G /\ IsValid m) (ValidOnly (m ᴳ· G)).
 Proof.
   intros *. unfold Basics.impl.
   hauto lq: on use: ValidOnlyStimesForward.
 Qed.
 Hint Rewrite <- ValidOnlyStimesForward' : suffices.
 
-Lemma DestOnlyUnionEquiv : forall (G1 G2 : ctx), ctx_DestOnly (G1 ᴳ+ G2) <-> ctx_DestOnly G1 /\ ctx_DestOnly G2.
+Lemma DestOnlyUnionEquiv : forall (G1 G2 : ctx), DestOnly (G1 ᴳ+ G2) <-> DestOnly G1 /\ DestOnly G2.
 Proof.
-  intros *. unfold ctx_DestOnly, ctx_union.
+  intros *. unfold DestOnly, ctx_union.
   apply merge_with_propagate_both.
   intros [xx|xh]. all: cbn. { sfirstorder. }
   intros b1 b2. unfold binding_union_dh. destruct b1, b2;
   destruct (type_eq_dec T T0), (mode_eq_dec n n0). all:sfirstorder.
 Qed.
 Hint Rewrite DestOnlyUnionEquiv : propagate_down.
-Lemma DestOnlyStimesEquiv : forall (m : mode) (G : ctx), ctx_DestOnly G <-> ctx_DestOnly (m ᴳ· G).
+Lemma DestOnlyStimesEquiv : forall (m : mode) (G : ctx), DestOnly G <-> DestOnly (m ᴳ· G).
 Proof.
-  intros *. unfold ctx_DestOnly, ctx_stimes.
+  intros *. unfold DestOnly, ctx_stimes.
   rewrite map_propagate_both'.
   { sfirstorder. }
-  unfold binding_IsDest.
+  unfold IsDest.
   hauto lq: on.
 Qed.
 Hint Rewrite <- DestOnlyStimesEquiv : propagate_down.
 
-Lemma mode_plus_not_lin : forall b1 b2, ~mode_IsLin (mode_plus b1 b2).
+Lemma mode_plus_not_lin : forall b1 b2, ~IsLin (mode_plus b1 b2).
 Proof.
   intros [[q1 [a1|]]|].
   2:{ cbn.  sauto q: on. }
@@ -307,37 +307,37 @@ Proof.
   inversion 1.
 Qed.
 
-Lemma IsLinNuWkIsLin : forall (m : mode), mode_IsLinNu m -> mode_IsLin m.
+Lemma IsLinNuWkIsLin : forall (m : mode), IsLinNu m -> IsLin m.
 Proof.
   intros *.
   sauto lq: on.
 Qed.
 
-Lemma IsLinNuWkIsLin' : forall (m : mode), Basics.impl (mode_IsLinNu m) (mode_IsLinNu m /\ mode_IsLin m).
+Lemma IsLinNuWkIsLin' : forall (m : mode), Basics.impl (IsLinNu m) (IsLinNu m /\ IsLin m).
 Proof.
   sfirstorder use: IsLinNuWkIsLin.
 Qed.
 Hint Rewrite IsLinNuWkIsLin' : saturate.
 
-Lemma IsLinWkIsValid : forall (m : mode), mode_IsLin m -> mode_IsValid m.
+Lemma IsLinWkIsValid : forall (m : mode), IsLin m -> IsValid m.
 Proof.
-  intros m H. destruct H. apply (mode_IsValidProof (Lin, a)).
+  intros m H. destruct H. apply (IsValidProof (Lin, a)).
 Qed.
 
-Lemma IsLinWkIsValid' : forall (m : mode), Basics.impl (mode_IsLin m) (mode_IsLin m /\ mode_IsValid m).
+Lemma IsLinWkIsValid' : forall (m : mode), Basics.impl (IsLin m) (IsLin m /\ IsValid m).
 Proof.
   sfirstorder use: IsLinWkIsValid.
 Qed.
 Hint Rewrite IsLinWkIsValid' : saturate.
 
-Lemma mode_plus_not_lin_nu : forall b1 b2, ~mode_IsLinNu (mode_plus b1 b2).
+Lemma mode_plus_not_lin_nu : forall b1 b2, ~IsLinNu (mode_plus b1 b2).
 Proof.
   intros b1 b2 h.
   apply IsLinNuWkIsLin in h.
   sfirstorder use: mode_plus_not_lin.
 Qed.
 
-Lemma LinOnlyUnionEquiv : forall (G1 G2 : ctx), ctx_LinOnly (G1 ᴳ+ G2) <-> ctx_LinOnly G1 /\ ctx_LinOnly G2 /\ G1 # G2.
+Lemma LinOnlyUnionEquiv : forall (G1 G2 : ctx), LinOnly (G1 ᴳ+ G2) <-> LinOnly G1 /\ LinOnly G2 /\ G1 # G2.
 Proof.
   intros *.
   apply merge_with_propagate_both_disjoint.
@@ -357,51 +357,51 @@ Proof.
 Qed.
 Hint Rewrite LinOnlyUnionEquiv : propagate_down.
 
-Lemma LinNuOnlyWkLinOnly : forall (G : ctx), ctx_LinNuOnly G -> ctx_LinOnly G.
+Lemma LinNuOnlyWkLinOnly : forall (G : ctx), LinNuOnly G -> LinOnly G.
 Proof.
   intros *.
   sfirstorder use: IsLinNuWkIsLin.
 Qed.
 
-Lemma LinOnlyWkValidOnly : forall (G : ctx), ctx_LinOnly G -> ctx_ValidOnly G.
+Lemma LinOnlyWkValidOnly : forall (G : ctx), LinOnly G -> ValidOnly G.
 Proof.
   intros *.
   sfirstorder use: IsLinWkIsValid.
 Qed.
 
-Lemma LinNuOnlyUnionEquiv : forall (G1 G2 : ctx), ctx_LinNuOnly (G1 ᴳ+ G2) <-> ctx_LinNuOnly G1 /\ ctx_LinNuOnly G2 /\ G1 # G2.
+Lemma LinNuOnlyUnionEquiv : forall (G1 G2 : ctx), LinNuOnly (G1 ᴳ+ G2) <-> LinNuOnly G1 /\ LinNuOnly G2 /\ G1 # G2.
 Proof.
   intros *.
   split.
   - intros h.
     assert (G1 # G2) as disj.
     { hauto lq: on use: LinOnlyUnionEquiv, LinNuOnlyWkLinOnly. }
-    assert (ctx_LinNuOnly G1 /\ ctx_LinNuOnly G2).
+    assert (LinNuOnly G1 /\ LinNuOnly G2).
     2:{ hauto lq: on. }
-    unfold ctx_LinNuOnly, ctx_union in *.
+    unfold LinNuOnly, ctx_union in *.
     eapply merge_with_propagate_backward_disjoint'.
     { apply disj. }
     eauto.
-  - intros h. unfold ctx_LinNuOnly, ctx_union in *.
+  - intros h. unfold LinNuOnly, ctx_union in *.
     apply merge_with_propagate_forward_disjoint.
     all: sfirstorder.
 Qed.
 Hint Rewrite LinNuOnlyUnionEquiv : propagate_down.
 
-Lemma LinNuOnlyStimesForward : forall (m : mode) (G : ctx), mode_IsLinNu m -> ctx_LinNuOnly G -> ctx_LinNuOnly (m ᴳ· G).
+Lemma LinNuOnlyStimesForward : forall (m : mode) (G : ctx), IsLinNu m -> LinNuOnly G -> LinNuOnly (m ᴳ· G).
 Proof.
   intros * linm linG.
-  unfold ctx_LinNuOnly in *.
+  unfold LinNuOnly in *.
   intros n b h.
   unfold ctx_stimes in h.
   rewrite map_MapsTo_iff in h. destruct h. destruct H.
   specialize (linG n x H). destruct n.
-  - unfold binding_stimes_var in H0. destruct x. subst. unfold binding_mode in *. unfold mode_IsLinNu in *. subst. unfold mode_times. cbn. reflexivity.
+  - unfold binding_stimes_var in H0. destruct x. subst. unfold binding_mode in *. unfold IsLinNu in *. subst. unfold mode_times. cbn. reflexivity.
   - unfold binding_stimes_dh in H0. destruct x; subst.
-    + unfold binding_mode in *. unfold mode_IsLinNu in *. subst. unfold mode_times. cbn. reflexivity.
-    + unfold binding_mode in *. unfold mode_IsLinNu in *. subst. unfold mode_times. cbn. reflexivity.
+    + unfold binding_mode in *. unfold IsLinNu in *. subst. unfold mode_times. cbn. reflexivity.
+    + unfold binding_mode in *. unfold IsLinNu in *. subst. unfold mode_times. cbn. reflexivity.
 Qed.
-Lemma LinNuOnlyStimesForward' : forall (m : mode) (G : ctx), Basics.impl (mode_IsLinNu m /\ ctx_LinNuOnly G) (ctx_LinNuOnly (m ᴳ· G)).
+Lemma LinNuOnlyStimesForward' : forall (m : mode) (G : ctx), Basics.impl (IsLinNu m /\ LinNuOnly G) (LinNuOnly (m ᴳ· G)).
 Proof.
   intros *. unfold Basics.impl.
   hauto lq: on use: LinNuOnlyStimesForward.
@@ -416,7 +416,7 @@ Proof.
   destruct H. tauto.
 Qed.
 
-Lemma LinNuOnlyStimesBackward : forall (m : mode) (G : ctx), ctx_LinNuOnly (m ᴳ· G) -> ctx_LinNuOnly G.
+Lemma LinNuOnlyStimesBackward : forall (m : mode) (G : ctx), LinNuOnly (m ᴳ· G) -> LinNuOnly G.
 Proof.
   intros *.
   intros islinNu.
@@ -425,24 +425,24 @@ Proof.
       | ʰ _ => binding_stimes_dh m
       end)
     as mf.
-    unfold ctx_LinNuOnly in *. intros n binding mapstoG. specialize (islinNu n (mf n binding)).
+    unfold LinNuOnly in *. intros n binding mapstoG. specialize (islinNu n (mf n binding)).
   assert ((m ᴳ· G) n = Some (mf n binding)).
     { eapply map_MapsTo_iff. exists binding. split. tauto. tauto. }
   specialize (islinNu H). unfold ctx_stimes in H. rewrite map_MapsTo_iff in H. destruct H. destruct H. destruct n; cbn in *. all: rewrite H in mapstoG; inversion mapstoG; subst. all:clear mf.
-  - destruct binding. unfold binding_stimes_var in *. unfold mode_times, mode_IsLinNu in *. destruct m, m0; cbn; try destruct p; try destruct p0.
+  - destruct binding. unfold binding_stimes_var in *. unfold mode_times, IsLinNu in *. destruct m, m0; cbn; try destruct p; try destruct p0.
     { unfold mul_times, age_times, ext_plus in *. destruct m, m0, a, a0; cbn; inversion islinNu; subst. rewrite H2, (n_plus_n0_eq_0_implies_n0_eq_0 n n0). all:trivial. }
     all: try congruence.
-  - destruct binding; unfold binding_stimes_dh in *; unfold mode_times, mode_IsLinNu in *; try rename n into m0; destruct m; destruct m0; cbn; try destruct p; try destruct p0; unfold mul_times, age_times, ext_plus in *; try rename n into m0; try destruct m; try destruct m0; try destruct a; try destruct a0; cbn; inversion islinNu; subst; rewrite H2.
+  - destruct binding; unfold binding_stimes_dh in *; unfold mode_times, IsLinNu in *; try rename n into m0; destruct m; destruct m0; cbn; try destruct p; try destruct p0; unfold mul_times, age_times, ext_plus in *; try rename n into m0; try destruct m; try destruct m0; try destruct a; try destruct a0; cbn; inversion islinNu; subst; rewrite H2.
     + rewrite (n_plus_n0_eq_0_implies_n0_eq_0 n0 n1). all:trivial.
     + rewrite (n_plus_n0_eq_0_implies_n0_eq_0 n n0). all:trivial.
 Qed.
-Lemma LinNuOnlyStimesBackward' : forall (m : mode) (G : ctx), Basics.impl (ctx_LinNuOnly (m ᴳ· G)) (ctx_LinNuOnly G).
+Lemma LinNuOnlyStimesBackward' : forall (m : mode) (G : ctx), Basics.impl (LinNuOnly (m ᴳ· G)) (LinNuOnly G).
 Proof.
   exact LinNuOnlyStimesBackward.
 Qed.
 Hint Rewrite LinNuOnlyStimesBackward' : propagate_down.
 
-Lemma FinAgeOnlyUnionBackward : forall (G1 G2 : ctx), ctx_FinAgeOnly (G1 ᴳ+ G2) -> ctx_FinAgeOnly G1 /\ ctx_FinAgeOnly G2.
+Lemma FinAgeOnlyUnionBackward : forall (G1 G2 : ctx), FinAgeOnly (G1 ᴳ+ G2) -> FinAgeOnly G1 /\ FinAgeOnly G2.
 Proof.
   intros *.
   apply merge_with_propagate_backward.
@@ -473,26 +473,26 @@ Proof.
     (* 2 goals left *)
     all: sfirstorder.
 Qed.
-Lemma FinAgeOnlyUnionBackward' : forall (G1 G2 : ctx), Basics.impl (ctx_FinAgeOnly (G1 ᴳ+ G2)) (ctx_FinAgeOnly G1 /\ ctx_FinAgeOnly G2).
+Lemma FinAgeOnlyUnionBackward' : forall (G1 G2 : ctx), Basics.impl (FinAgeOnly (G1 ᴳ+ G2)) (FinAgeOnly G1 /\ FinAgeOnly G2).
 Proof.
   exact FinAgeOnlyUnionBackward.
 Qed.
 Hint Rewrite FinAgeOnlyUnionBackward' : propagate_down.
 
-Lemma FinAgeOnlyUnionForward : forall (G1 G2 : ctx), (ctx_FinAgeOnly G1 /\ ctx_FinAgeOnly G2 /\ G1 # G2) -> ctx_FinAgeOnly (G1 ᴳ+ G2).
+Lemma FinAgeOnlyUnionForward : forall (G1 G2 : ctx), (FinAgeOnly G1 /\ FinAgeOnly G2 /\ G1 # G2) -> FinAgeOnly (G1 ᴳ+ G2).
 Proof.
-  intros * h. unfold ctx_union, ctx_FinAgeOnly.
+  intros * h. unfold ctx_union, FinAgeOnly.
   apply merge_with_propagate_forward_disjoint.
   all: sfirstorder.
 Qed.
-Lemma FinAgeOnlyUnionForward' : forall (G1 G2 : ctx), Basics.impl (ctx_FinAgeOnly G1 /\ ctx_FinAgeOnly G2 /\ G1 # G2) (ctx_FinAgeOnly (G1 ᴳ+ G2)).
+Lemma FinAgeOnlyUnionForward' : forall (G1 G2 : ctx), Basics.impl (FinAgeOnly G1 /\ FinAgeOnly G2 /\ G1 # G2) (FinAgeOnly (G1 ᴳ+ G2)).
 Proof.
   intros *. unfold Basics.impl.
   hauto lq: on use: FinAgeOnlyUnionForward.
 Qed.
 Hint Rewrite <- FinAgeOnlyUnionForward' : suffices.
 
-Lemma LinOnlyStimesBackward : forall (m : mode) (G : ctx), ctx_LinOnly (m ᴳ· G) -> ctx_LinOnly G.
+Lemma LinOnlyStimesBackward : forall (m : mode) (G : ctx), LinOnly (m ᴳ· G) -> LinOnly G.
 Proof.
   intros *.
   intros islin.
@@ -501,7 +501,7 @@ Proof.
       | ʰ _ => binding_stimes_dh m
       end)
     as mf.
-    unfold ctx_LinOnly in *. intros n binding mapstoG. specialize (islin n (mf n binding)).
+    unfold LinOnly in *. intros n binding mapstoG. specialize (islin n (mf n binding)).
   assert ((m ᴳ· G) n = Some (mf n binding)).
     { eapply map_MapsTo_iff. exists binding. split. tauto. tauto. }
   specialize (islin H). unfold ctx_stimes in H. rewrite map_MapsTo_iff in H. destruct H. destruct H. destruct n; cbn in *. all: rewrite H in mapstoG; inversion mapstoG; subst. all:clear mf.
@@ -514,16 +514,16 @@ Proof.
     all: inversion islin.
     { unfold mul_times, age_times, ext_plus in *. destruct m0, m1, a, a0; cbn; try constructor. all: inversion islin. }
 Qed.
-Lemma LinOnlyStimesBackward' : forall (m : mode) (G : ctx), Basics.impl (ctx_LinOnly (m ᴳ· G)) (ctx_LinOnly G).
+Lemma LinOnlyStimesBackward' : forall (m : mode) (G : ctx), Basics.impl (LinOnly (m ᴳ· G)) (LinOnly G).
 Proof.
   exact LinOnlyStimesBackward.
 Qed.
 Hint Rewrite LinOnlyStimesBackward' : propagate_down.
 
-Lemma LinOnlyStimesForward : forall (m : mode) (G : ctx), mode_IsLin m -> ctx_LinOnly G -> ctx_LinOnly (m ᴳ· G).
+Lemma LinOnlyStimesForward : forall (m : mode) (G : ctx), IsLin m -> LinOnly G -> LinOnly (m ᴳ· G).
 Proof.
   intros * validm linG.
-  unfold ctx_LinOnly in *.
+  unfold LinOnly in *.
   intros n b h.
   unfold ctx_stimes in h.
   rewrite map_MapsTo_iff in h. destruct h. destruct H.
@@ -531,14 +531,14 @@ Proof.
   - unfold binding_stimes_var in H0. destruct x. subst. unfold binding_mode in *. destruct m, m0; try destruct p; try destruct p0; try destruct m; try destruct m0; unfold mode_times, mul_times in *; cbn; try constructor; try inversion linG; try inversion validm.
   - unfold binding_stimes_dh in H0. destruct x; subst; unfold binding_mode in *; try rename n into m0; destruct m, m0; try destruct p; try destruct p0; try destruct m; try destruct m0; unfold mode_times, mul_times in *; cbn; try constructor; try inversion linG; try inversion validm.
 Qed.
-Lemma LinOnlyStimesForward' : forall (m : mode) (G : ctx), Basics.impl (mode_IsLin m /\ ctx_LinOnly G) (ctx_LinOnly (m ᴳ· G)).
+Lemma LinOnlyStimesForward' : forall (m : mode) (G : ctx), Basics.impl (IsLin m /\ LinOnly G) (LinOnly (m ᴳ· G)).
 Proof.
   intros *. unfold Basics.impl.
   hauto lq: on use: LinOnlyStimesForward.
 Qed.
 Hint Rewrite <- LinOnlyStimesForward' : suffices.
 
-Lemma FinAgeOnlyStimesBackward : forall (m : mode) (G : ctx), ctx_FinAgeOnly (m ᴳ· G) -> ctx_FinAgeOnly G.
+Lemma FinAgeOnlyStimesBackward : forall (m : mode) (G : ctx), FinAgeOnly (m ᴳ· G) -> FinAgeOnly G.
 Proof.
   intros *.
   intros isfinAge.
@@ -547,7 +547,7 @@ Proof.
       | ʰ _ => binding_stimes_dh m
       end)
     as mf.
-    unfold ctx_FinAgeOnly in *. intros n binding mapstoG. specialize (isfinAge n (mf n binding)).
+    unfold FinAgeOnly in *. intros n binding mapstoG. specialize (isfinAge n (mf n binding)).
   assert ((m ᴳ· G) n = Some (mf n binding)).
     { eapply map_MapsTo_iff. exists binding. split. tauto. tauto. }
   specialize (isfinAge H). unfold ctx_stimes in H. rewrite map_MapsTo_iff in H. destruct H. destruct H. destruct n; cbn in *. all: rewrite H in mapstoG; inversion mapstoG; subst. all:clear mf.
@@ -560,16 +560,16 @@ Proof.
     all: inversion isfinAge.
     { unfold mul_times, age_times, ext_plus in *. destruct m0, m1, a, a0; cbn; try constructor. all: inversion isfinAge. }
 Qed.
-Lemma FinAgeOnlyStimesBackward' : forall (m : mode) (G : ctx), Basics.impl (ctx_FinAgeOnly (m ᴳ· G)) (ctx_FinAgeOnly G).
+Lemma FinAgeOnlyStimesBackward' : forall (m : mode) (G : ctx), Basics.impl (FinAgeOnly (m ᴳ· G)) (FinAgeOnly G).
 Proof.
   exact FinAgeOnlyStimesBackward.
 Qed.
 Hint Rewrite FinAgeOnlyStimesBackward' : propagate_down.
 
-Lemma FinAgeOnlyStimesForward : forall (m : mode) (G : ctx), mode_IsFinAge m -> ctx_FinAgeOnly G -> ctx_FinAgeOnly (m ᴳ· G).
+Lemma FinAgeOnlyStimesForward : forall (m : mode) (G : ctx), IsFinAge m -> FinAgeOnly G -> FinAgeOnly (m ᴳ· G).
 Proof.
   intros * validm finAgeG.
-  unfold ctx_FinAgeOnly in *.
+  unfold FinAgeOnly in *.
   intros n b h.
   unfold ctx_stimes in h.
   rewrite map_MapsTo_iff in h. destruct h. destruct H.
@@ -577,7 +577,7 @@ Proof.
   - unfold binding_stimes_var in H0. destruct x. subst. unfold binding_mode in *. destruct m, m0; try destruct p; try destruct p0; try destruct a; try destruct a0; unfold mode_times, age_times in *; cbn; try constructor; try inversion finAgeG; try inversion validm.
   - unfold binding_stimes_dh in H0. destruct x; subst; unfold binding_mode in *; try rename n into m0; destruct m, m0; try destruct p; try destruct p0; try destruct a; try destruct a0; unfold mode_times, age_times in *; cbn; try constructor; try inversion finAgeG; try inversion validm.
 Qed.
-Lemma FinAgeOnlyStimesForward' : forall (m : mode) (G : ctx), Basics.impl (mode_IsFinAge m /\ ctx_FinAgeOnly G) (ctx_FinAgeOnly (m ᴳ· G)).
+Lemma FinAgeOnlyStimesForward' : forall (m : mode) (G : ctx), Basics.impl (IsFinAge m /\ FinAgeOnly G) (FinAgeOnly (m ᴳ· G)).
 Proof.
   intros *. unfold Basics.impl.
   hauto lq: on use: FinAgeOnlyStimesForward.
@@ -590,7 +590,7 @@ Proof.
     they ought to because we can't rewrite under foralls. I [aspiwack]
     am however unwilling to spend the time and find a better way,
     copy-paste will do. *)
-  intros *. unfold ctx_Disjoint, ctx_stimes.
+  intros *. unfold Disjoint, ctx_stimes.
   split.
   - intros h x.
     specialize (h x).
@@ -604,7 +604,7 @@ Hint Rewrite DisjointStimesLeftEquiv : propagate_down.
 
 Lemma DisjointStimesRightEquiv : forall (m : mode) (D D' : ctx), D # (m ᴳ· D') <-> D # D'.
 Proof.
-  intros *. unfold ctx_Disjoint, ctx_stimes.
+  intros *. unfold Disjoint, ctx_stimes.
   split.
   - intros h x.
     specialize (h x).
@@ -618,7 +618,7 @@ Hint Rewrite DisjointStimesRightEquiv : propagate_down.
 
 Lemma DisjointMinusLeftEquiv : forall (D D' : ctx), D # D' <-> ((ᴳ- D)) # D'.
 Proof.
-  intros *. unfold ctx_Disjoint, ctx_minus.
+  intros *. unfold Disjoint, ctx_minus.
   split.
   - intros h x.
     rewrite In_map_iff.
@@ -632,7 +632,7 @@ Hint Rewrite <- DisjointMinusLeftEquiv : propagate_down.
 
 Lemma DisjointInvMinusLeftEquiv : forall (D D' : ctx), D # D' <-> ((ᴳ-⁻¹ D)) # D'.
 Proof.
-  intros *. unfold ctx_Disjoint, ctx_invminus.
+  intros *. unfold Disjoint, ctx_invminus.
   split.
   - intros h x.
     rewrite In_map_iff.
@@ -645,7 +645,7 @@ Qed.
 
 Lemma DisjointMinusRightEquiv : forall (D D' : ctx), D # D' <-> D # ((ᴳ-D')).
 Proof.
-  intros *. unfold ctx_Disjoint, ctx_minus.
+  intros *. unfold Disjoint, ctx_minus.
   split.
   - intros h x.
     rewrite In_map_iff.
@@ -659,7 +659,7 @@ Hint Rewrite <- DisjointMinusRightEquiv : propagate_down.
 
 Lemma DisjointInvMinusRightEquiv : forall (D D' : ctx), D # D' <-> D # ((ᴳ-⁻¹D')).
 Proof.
-  intros *. unfold ctx_Disjoint, ctx_invminus.
+  intros *. unfold Disjoint, ctx_invminus.
   split.
   - intros h x.
     rewrite In_map_iff.
@@ -672,7 +672,7 @@ Qed.
 
 Lemma DisjointNestedLeftEquiv : forall (D D' D'' : ctx), (D ᴳ+ D') # D'' <-> D # D'' /\ D' # D''.
 Proof.
-  intros *. unfold ctx_Disjoint, ctx_union.
+  intros *. unfold Disjoint, ctx_union.
   split.
   - intros h.
     split.
@@ -689,7 +689,7 @@ Hint Rewrite DisjointNestedLeftEquiv : propagate_down.
 Lemma DisjointNestedRightEquiv : forall (D D' D'' : ctx), D # (D' ᴳ+ D'') <-> D # D' /\ D # D''.
 Proof.
 Proof.
-  intros *. unfold ctx_Disjoint, ctx_union.
+  intros *. unfold Disjoint, ctx_union.
   split.
   - intros h.
     split.
@@ -705,38 +705,38 @@ Hint Rewrite DisjointNestedRightEquiv : propagate_down.
 
 Lemma DisjointCommutative : forall (G1 G2 : ctx), G1 # G2 <-> G2 # G1.
 Proof.
-  intros *. unfold ctx_Disjoint.
+  intros *. unfold Disjoint.
   sfirstorder.
 Qed.
 
-Lemma EmptyIsLinOnly : ctx_LinOnly ᴳ{}.
+Lemma EmptyIsLinOnly : LinOnly ᴳ{}.
 Proof.
-  scongruence unfold: ctx_LinOnly.
+  scongruence unfold: LinOnly.
 Qed.
 
-Lemma EmptyIsFinAgeOnly : ctx_FinAgeOnly ᴳ{}.
+Lemma EmptyIsFinAgeOnly : FinAgeOnly ᴳ{}.
 Proof.
-  scongruence unfold: ctx_FinAgeOnly.
+  scongruence unfold: FinAgeOnly.
 Qed.
 
-Lemma Emptybinding_IsDestOnly : ctx_DestOnly ᴳ{}.
+Lemma EmptyIsDestOnly : DestOnly ᴳ{}.
 Proof.
-  sauto q: on unfold: ctx_DestOnly.
+  sauto q: on unfold: DestOnly.
 Qed.
 
 Lemma EmptyIsDisjointLeft : forall (G : ctx), ᴳ{} # G.
 Proof.
-  sauto q: on unfold: ctx_Disjoint.
+  sauto q: on unfold: Disjoint.
 Qed.
 
-Lemma EmptyIsDisjointRight : forall (G : ctx), ctx_Disjoint G ᴳ{}.
+Lemma EmptyIsDisjointRight : forall (G : ctx), Disjoint G ᴳ{}.
 Proof.
-  sauto q: on unfold: ctx_Disjoint.
+  sauto q: on unfold: Disjoint.
 Qed.
 
-Lemma EmptyIsDisposableOnly : ctx_DisposableOnly ᴳ{}.
+Lemma EmptyIsDisposableOnly : DisposableOnly ᴳ{}.
 Proof.
-  sauto q: on unfold: ctx_DisposableOnly.
+  sauto q: on unfold: DisposableOnly.
 Qed.
 
 Lemma StimesEmptyEq : forall (m : mode), m ᴳ· ᴳ{} = ᴳ{}.
@@ -790,17 +790,17 @@ Proof.
 Qed.
 Hint Rewrite <- UnionIdentityLeft : canonalize.
 
-Lemma DisjointDestOnlyVar : forall (G : ctx) (x : var) (m : mode) (T : type), ctx_DestOnly G -> G # (ᴳ{ x : m ‗ T}).
+Lemma DisjointDestOnlyVar : forall (G : ctx) (x : var) (m : mode) (T : type), DestOnly G -> G # (ᴳ{ x : m ‗ T}).
 Proof.
   intros * destonly.
-  unfold ctx_DestOnly, ctx_Disjoint in *.
+  unfold DestOnly, Disjoint in *.
   intros n inG inSing.
   unfold In, Fun.In in *.
   destruct inG as (binding & mapsto).
   specialize (destonly n binding mapsto).
   unfold ctx_singleton in inSing. destruct inSing. rewrite singleton_MapsTo_iff in H.
   inversion H; subst.
-  unfold binding_IsDest in destonly. assumption.
+  unfold IsDest in destonly. assumption.
 Qed.
 
 Lemma mode_plus_commutative : forall (m n: mode), mode_plus m n = mode_plus n m.
@@ -980,23 +980,23 @@ Hint Rewrite StimesUnionDistributive : canonalize.
 
 Lemma MinusUnionDistributive : forall (G1 G2 : ctx), G1 # G2 ->(ᴳ- (G1 ᴳ+ G2)) = (ᴳ-G1) ᴳ+ (ᴳ-G2).
 Proof.
-  intros * Disjoint.
+  intros * DisjointG1G2.
   apply Finitely.ext_eq.
   intros n. unfold ctx_minus, ctx_union.
   unfold map, merge_with, merge, Fun.map, Fun.merge, Fun.on_conflict_do.
   destruct (In_dec n G1), (In_dec n G2).
-  { unfold ctx_Disjoint in Disjoint. specialize (Disjoint n H H0). contradiction. }
+  { unfold Disjoint in DisjointG1G2. specialize (DisjointG1G2 n H H0). contradiction. }
   all: destruct n; try destruct H as (binding1 & mapstoG1); try destruct H0 as (binding2 & mapstoG2); cbn; try rewrite nIn_iff_nMapsTo in H; try rewrite nIn_iff_nMapsTo in H0; try rewrite mapstoG1; try rewrite mapstoG2; try rewrite H; try rewrite H0; cbn; trivial.
 Qed.
 
 Lemma InvMinusUnionDistributive : forall (G1 G2 : ctx), G1 # G2 ->(ᴳ-⁻¹ (G1 ᴳ+ G2)) = (ᴳ-⁻¹G1) ᴳ+ (ᴳ-⁻¹G2).
 Proof.
-  intros * Disjoint.
+  intros * DisjointG1G2.
   apply Finitely.ext_eq.
   intros n. unfold ctx_invminus, ctx_union.
   unfold map, merge_with, merge, Fun.map, Fun.merge, Fun.on_conflict_do.
   destruct (In_dec n G1), (In_dec n G2).
-  { unfold ctx_Disjoint in Disjoint. specialize (Disjoint n H H0). contradiction. }
+  { unfold Disjoint in DisjointG1G2. specialize (DisjointG1G2 n H H0). contradiction. }
   all: destruct n; try destruct H as (binding1 & mapstoG1); try destruct H0 as (binding2 & mapstoG2); cbn; try rewrite nIn_iff_nMapsTo in H; try rewrite nIn_iff_nMapsTo in H0; try rewrite mapstoG1; try rewrite mapstoG2; try rewrite H; try rewrite H0; cbn; trivial.
 Qed.
 
@@ -1171,24 +1171,24 @@ Proof.
   - left. rewrite hvarsMinusEq. assumption.
 Qed.
 
-Lemma hvars_DisjointToDisjoint : forall (D D' : ctx), ctx_DestOnly D -> hvarsᴳ(D) ## hvarsᴳ(D') -> D # D'.
+Lemma HDisjointToDisjoint : forall (D D' : ctx), DestOnly D -> hvarsᴳ(D) ## hvarsᴳ(D') -> D # D'.
 Proof.
   intros * DestOnlyD hvarsDisjoint.
-  unfold ctx_Disjoint. intros n inD inD'. unfold In, Fun.In in *. destruct n.
-  - unfold ctx_DestOnly, binding_IsDest in DestOnlyD. destruct inD as (binding & inD); specialize (DestOnlyD (name_Var x) binding inD); cbn in DestOnlyD. assumption.
-  - rewrite <- hvars_spec in inD, inD'. unfold hvars_Disjoint in hvarsDisjoint.
+  unfold Disjoint. intros n inD inD'. unfold In, Fun.In in *. destruct n.
+  - unfold DestOnly, IsDest in DestOnlyD. destruct inD as (binding & inD); specialize (DestOnlyD (name_Var x) binding inD); cbn in DestOnlyD. assumption.
+  - rewrite <- hvars_spec in inD, inD'. unfold HDisjoint in hvarsDisjoint.
     assert (NatSet.In h (NatSet.inter hvarsᴳ(D) hvarsᴳ(D'))).
       { apply NatSet.inter_spec. split; assumption. }
     unfold NatSet.Empty in hvarsDisjoint. specialize (hvarsDisjoint h). congruence.
 Qed.
 
-Lemma DisjointTohvars_Disjoint : forall (D D' : ctx), D # D' -> hvarsᴳ(D) ## hvarsᴳ(D').
+Lemma DisjointToHDisjoint : forall (D D' : ctx), D # D' -> hvarsᴳ(D) ## hvarsᴳ(D').
 Proof.
-  intros * Disjoint.
-  unfold hvars_Disjoint. unfold NatSet.Empty. intros h HinInter.
+  intros * DisjointDDp.
+  unfold HDisjoint. unfold NatSet.Empty. intros h HinInter.
   rewrite NatSetFacts.inter_iff in HinInter. destruct HinInter as (inD & inD').
   rewrite hvars_spec in inD, inD'. rewrite <- In_iff_exists_Some in inD, inD'.
-  unfold ctx_Disjoint in Disjoint. specialize (Disjoint (name_DH h) inD inD'). assumption.
+  unfold Disjoint in DisjointDDp. specialize (DisjointDDp (name_DH h) inD inD'). assumption.
 Qed.
 
 Lemma not_lt_le : forall (x y : nat),
@@ -1213,16 +1213,16 @@ Proof.
   unfold hvars_ctx, hvars_dom, ctx_empty. rewrite dom_empty_eq_nil. reflexivity.
 Qed.
 
-Lemma EmptyIshvars_DisjointRight : forall (H : hvars), H ## NatSet.empty.
+Lemma EmptyIsHDisjointRight : forall (H : hvars), H ## NatSet.empty.
 Proof.
-  intros H. unfold hvars_Disjoint. unfold NatSet.Empty. intros h Hin. rewrite NatSet.inter_spec in Hin. destruct Hin. inversion H1.
+  intros H. unfold HDisjoint. unfold NatSet.Empty. intros h Hin. rewrite NatSet.inter_spec in Hin. destruct Hin. inversion H1.
 Qed.
-Lemma EmptyIshvars_DisjointLeft : forall (H : hvars), NatSet.empty ## H.
+Lemma EmptyIsHDisjointLeft : forall (H : hvars), NatSet.empty ## H.
 Proof.
-  intros H. unfold hvars_Disjoint. unfold NatSet.Empty. intros h Hin. rewrite NatSet.inter_spec in Hin. destruct Hin. inversion H0.
+  intros H. unfold HDisjoint. unfold NatSet.Empty. intros h Hin. rewrite NatSet.inter_spec in Hin. destruct Hin. inversion H0.
 Qed.
 
-Lemma IsSubtype_refl : forall (m : mode), mode_IsSubtype m m.
+Lemma IsSubtype_refl : forall (m : mode), ModeSubtype m m.
 Proof.
   intros m. sauto lq: on.
 Qed.
@@ -1239,13 +1239,13 @@ Proof.
     - exact (name_eq_dec).
 Qed.
 
-Lemma IncompatibleVarDestOnly : forall (D : ctx) (x : var) (m : mode) (T : type), ctx_DestOnly D -> ~ctx_CompatibleVar D x (ₓ m ‗ T).
+Lemma IncompatibleVarDestOnlyD : forall (D : ctx) (x : var) (m : mode) (T : type), DestOnly D -> ~CompatibleVar D x (ₓ m ‗ T).
 Proof.
-  intros * DestOnly CompatibleVar. destruct CompatibleVar as (inD & CompatibleVar).
-  unfold ctx_DestOnly, binding_IsDest in DestOnly. unfold ctx_CompatibleVar in CompatibleVar. destruct (dom(D)) eqn:eDomD.
+  intros * DestOnlyD CompatibleVar. destruct CompatibleVar as (inD & CompatibleVar).
+  unfold DestOnly, IsDest in DestOnlyD. unfold CompatibleVar in CompatibleVar. destruct (dom(D)) eqn:eDomD.
   - rewrite <- dom_spec in inD. rewrite eDomD in inD. inversion inD.
   - assert (List.In n (dom D)). { rewrite eDomD. apply in_eq. }
-    rewrite dom_spec in H. destruct H as (binding & mapstoD). destruct n. specialize (DestOnly (ˣ x0) binding mapstoD). assumption. apply In_iff_exists_Some in inD; destruct inD as (binding' & mapstoD'). specialize (DestOnly (ˣ x) binding' mapstoD'). simpl in DestOnly. assumption.
+    rewrite dom_spec in H. destruct H as (binding & mapstoD). destruct n. specialize (DestOnlyD (ˣ x0) binding mapstoD). assumption. apply In_iff_exists_Some in inD; destruct inD as (binding' & mapstoD'). specialize (DestOnlyD (ˣ x) binding' mapstoD'). simpl in DestOnlyD. assumption.
 Qed. *)
 
 Lemma MinusSingletonEq : forall (h : hvar) (T : type) (n : mode), (ᴳ- ᴳ{+ h : ¹ν ⌊ T ⌋ n}) = ᴳ{- h : T ‗ n }.
@@ -1321,15 +1321,15 @@ Proof.
   rewrite dom_singleton_eq. reflexivity.
 Qed.
 
-Lemma SingletonDestIsDestOnly : forall (h : hvar) (m n : mode) (T : type), ctx_DestOnly ᴳ{+ h : m ⌊ T ⌋ n}.
+Lemma SingletonDestIsDestOnly : forall (h : hvar) (m n : mode) (T : type), DestOnly ᴳ{+ h : m ⌊ T ⌋ n}.
 Proof.
-  unfold ctx_DestOnly, ctx_singleton, binding_IsDest. intros * mapsto.
+  unfold DestOnly, ctx_singleton, IsDest. intros * mapsto.
   apply singleton_MapsTo_iff in mapsto. pose proof mapsto as mapsto'. apply eq_sigT_fst in mapsto. destruct x; try congruence. inversion mapsto. rewrite <- H0 in *. apply inj_pair2_eq_dec in mapsto'. rewrite <- mapsto' in *. trivial. exact name_eq_dec.
 Qed.
 
-Lemma SingletonVarIsVarOnly : forall (x : var) (m : mode) (T : type), ctx_VarOnly ᴳ{ x : m ‗ T}.
+Lemma SingletonVarIsVarOnly : forall (x : var) (m : mode) (T : type), VarOnly ᴳ{ x : m ‗ T}.
 Proof.
-  unfold ctx_VarOnly, ctx_singleton, binding_IsVar. intros * mapsto.
+  unfold VarOnly, ctx_singleton, IsVar. intros * mapsto.
   apply singleton_MapsTo_iff in mapsto. pose proof mapsto as mapsto'. apply eq_sigT_fst in mapsto. destruct x0; try congruence. inversion mapsto. rewrite <- H0 in *. apply inj_pair2_eq_dec in mapsto'. trivial. exact name_eq_dec.
 Qed.
 
@@ -1339,37 +1339,12 @@ Proof.
   apply Finitely.dom_nil_is_empty.
 Qed.
 
-Lemma SubsetDisjoint : forall (H1 H2 H3 : hvars), NatSet.Subset H1 H2 -> hvars_Disjoint H2 H3 -> hvars_Disjoint H1 H3.
+Lemma SubsetDisjoint : forall (H1 H2 H3 : hvars), NatSet.Subset H1 H2 -> HDisjoint H2 H3 -> HDisjoint H1 H3.
 Proof.
-  intros * H1H2 H2H3. unfold hvars_Disjoint, NatSet.Subset, NatSet.Empty in *.
+  intros * H1H2 H2H3. unfold HDisjoint, NatSet.Subset, NatSet.Empty in *.
   intros h. specialize (H1H2 h). specialize (H2H3 h).
   intros HinInter. apply NatSet.inter_spec in HinInter. destruct HinInter as [H1h H3h]. specialize (H1H2 H1h). destruct H2H3. apply NatSet.inter_spec. split; assumption.
 Qed.
-
-(* Lemma CompatibleLinFinOnlyIsExact : forall (D : ctx) (h : hvar) (T : type) (n : mode), ctx_LinOnly D -> ctx_FinAgeOnly D -> ctx_CompatibleDH D h (₊ ¹ν ⌊ T ⌋ n) -> (forall x, D x = ᴳ{+ h : ¹ν ⌊ T ⌋ n} x).
-Proof.
-  intros * LinOnly FinAgeOnly CompatibleDH.
-  unfold ctx_CompatibleDH in CompatibleDH. destruct CompatibleDH as (inD & CompatibleDH).
-  intros nam. destruct (name_eq_dec nam (ʰ h)).
-    + rewrite e in *. unfold ctx_singleton. rewrite singleton_MapsKeyTo. rewrite In_iff_exists_Some in inD.
-      destruct inD as (binding & inD). specialize (CompatibleDH (ʰ h) binding inD). simpl in CompatibleDH. destruct (NatSetFacts.eq_dec h h) in CompatibleDH.
-      2:{ congruence. }
-      destruct binding eqn: ebinding in CompatibleDH.
-      { destruct CompatibleDH as (sub & e1 & e2). subst.
-        assert (¹ν = m). { inversion sub. inversion H1. inversion H3. reflexivity. }
-        rewrite <- H in inD; assumption.
-      }
-      { contradiction. }
-    + specialize (CompatibleDH nam). destruct (D nam) eqn:mapsto.
-      { specialize (CompatibleDH b eq_refl). destruct nam.
-        { unfold ctx_LinOnly in LinOnly. specialize (LinOnly (ˣ x) b mapsto). inversion LinOnly. inversion CompatibleDH. destruct b; congruence. }
-        { destruct (NatSetFacts.eq_dec h h0).
-          congruence.
-          unfold ctx_LinOnly in LinOnly. specialize (LinOnly (ʰ h0) b mapsto). inversion LinOnly. inversion CompatibleDH.
-        }
-      }
-      { unfold ctx_singleton. symmetry. apply singleton_nMapsTo_iff. symmetry. assumption. }
-Qed. *)
 
 Lemma InUnionLeft : forall (D1 D2 : ctx) (n : name), In n D1 -> In n (D1 ᴳ+ D2).
 Proof.
@@ -1402,10 +1377,10 @@ Lemma NotInEquivDisjointSingleton : forall (G : ctx) (n : name) (binding : bindi
 Proof.
   intros *.
   split.
-  - intros NotIn. unfold ctx_Disjoint. intros n'. intros InG. destruct (name_eq_dec n n'). rewrite e in *. congruence. intros inSing. unfold ctx_singleton in inSing. rewrite <- singleton_nMapsTo_iff with (x := n) (discr := name_eq_dec) (v := binding) in n0. rewrite In_iff_exists_Some in inSing. destruct inSing. congruence.
-  - intros Disjoint. unfold ctx_Disjoint in Disjoint. intros InG.
+  - intros NotIn. unfold Disjoint. intros n'. intros InG. destruct (name_eq_dec n n'). rewrite e in *. congruence. intros inSing. unfold ctx_singleton in inSing. rewrite <- singleton_nMapsTo_iff with (x := n) (discr := name_eq_dec) (v := binding) in n0. rewrite In_iff_exists_Some in inSing. destruct inSing. congruence.
+  - intros DisjointGSing. unfold Disjoint in DisjointGSing. intros InG.
     assert (In n (ctx_singleton n binding)). { apply In_singleton_iff; reflexivity. }
-    specialize (Disjoint n InG H). assumption.
+    specialize (DisjointGSing n InG H). assumption.
 Qed.
 
 Lemma NotInUnionForward: forall (G1 G2 : ctx) (n : name), ~In n G1 -> ~In n G2 -> ~In n (G1 ᴳ+ G2).
@@ -1413,68 +1388,68 @@ Proof.
   intros * NotIn1 NotIn2 InUnion. unfold ctx_union in InUnion. apply In_merge_iff in InUnion. destruct InUnion. all:congruence.
 Qed.
 
-Lemma DestOnlyWkNoVar : forall (D : ctx), ctx_DestOnly D -> ctx_NoVar D.
+Lemma DestOnlyWkNoVar : forall (D : ctx), DestOnly D -> NoVar D.
 Proof.
-  intros * H. unfold ctx_DestOnly in H. unfold ctx_NoVar. intros nam b mapstoD. specialize (H nam b mapstoD). destruct nam. { inversion H. } { intros contra. inversion contra. }
+  intros * H. unfold DestOnly in H. unfold NoVar. intros nam b mapstoD. specialize (H nam b mapstoD). destruct nam. { inversion H. } { intros contra. inversion contra. }
 Qed.
 
-Lemma DisposableOnlyWkVarOnly : forall (P : ctx), ctx_DisposableOnly P -> ctx_VarOnly P.
+Lemma DisposableOnlyWkVarOnly : forall (P : ctx), DisposableOnly P -> VarOnly P.
 Proof.
-  intros * H. unfold ctx_DisposableOnly in H. unfold ctx_VarOnly. intros nam b mapstoP. specialize (H nam b mapstoP). unfold binding_IsDisposable in H. destruct nam. 2:{ contradiction. } unfold binding_IsVar. tauto.
+  intros * H. unfold DisposableOnly in H. unfold VarOnly. intros nam b mapstoP. specialize (H nam b mapstoP). unfold IsDisposable in H. destruct nam. 2:{ contradiction. } unfold IsVar. tauto.
 Qed.
 
-Lemma SimplifyDisposableInTyC: forall (P D : ctx), ctx_DisposableOnly P -> ctx_DestOnly (P ᴳ+ D) -> (P ᴳ+ D) = D.
+Lemma SimplifyDisposableInTyC: forall (P D : ctx), DisposableOnly P -> DestOnly (P ᴳ+ D) -> (P ᴳ+ D) = D.
 Proof.
   intros * DisposP DestOnlyPuD.
   assert (P = ᴳ{}) as Pempty.
   { apply ext_eq. intros n. destruct (In_dec n P) as [[y h_inP]|h_ninP].
-    - unfold ctx_DisposableOnly in DisposP. specialize (DisposP n y h_inP). unfold binding_IsDisposable in DisposP.
-      unfold ctx_DestOnly in DestOnlyPuD. assert (In n P) as inP. { exists y. assumption. } assert (In n (P ᴳ+ D)) as InPuD. { apply InUnionLeft. assumption. } destruct InPuD as (y' & mapstoPuD). specialize (DestOnlyPuD n y' mapstoPuD). unfold binding_IsDest in DestOnlyPuD. destruct n; contradiction.
+    - unfold DisposableOnly in DisposP. specialize (DisposP n y h_inP). unfold IsDisposable in DisposP.
+      unfold DestOnly in DestOnlyPuD. assert (In n P) as inP. { exists y. assumption. } assert (In n (P ᴳ+ D)) as InPuD. { apply InUnionLeft. assumption. } destruct InPuD as (y' & mapstoPuD). specialize (DestOnlyPuD n y' mapstoPuD). unfold IsDest in DestOnlyPuD. destruct n; contradiction.
     - apply nIn_iff_nMapsTo. assumption.
   }
   rewrite Pempty. symmetry. apply UnionIdentityLeft.
 Qed.
 
-Lemma VarOnlyNoVarUnionIsDisjoint : forall (D1 G2 : ctx), ctx_VarOnly D1 -> ctx_NoVar G2 -> D1 # G2.
+Lemma VarOnlyNoVarUnionIsDisjoint : forall (P1 G2 : ctx), VarOnly P1 -> NoVar G2 -> P1 # G2.
 Proof.
-  intros * VarOnly NoVar. unfold ctx_Disjoint. intros nam inD1 inG2. unfold ctx_VarOnly, ctx_NoVar, Fun.In, binding_IsVar in *. destruct inD1; specialize (VarOnly nam x H). destruct inG2; specialize (NoVar nam x0 H0). destruct nam; simpl in *; congruence.
+  intros * VarOnlyP NoVarG. unfold Disjoint. intros nam inP1 inG2. unfold VarOnly, NoVar, Fun.In, IsVar in *. destruct inP1; specialize (VarOnlyP nam x H). destruct inG2; specialize (NoVarG nam x0 H0). destruct nam; simpl in *; congruence.
 Qed.
 
-Lemma DestOnlyAtXIsNone : forall (D : ctx) (x : var), ctx_DestOnly D -> D (ˣ x) = None.
+Lemma DestOnlyAtXIsNone : forall (D : ctx) (x : var), DestOnly D -> D (ˣ x) = None.
 Proof.
-  intros * DestOnly. unfold ctx_DestOnly in DestOnly. specialize (DestOnly (ˣ x)).
+  intros * DestOnlyD. unfold DestOnly in DestOnlyD. specialize (DestOnlyD (ˣ x)).
   destruct (List.In_dec name_eq_dec (ˣ x) (dom D)).
     2:{ rewrite dom_spec in n. rewrite nIn_iff_nMapsTo in n. assumption. }
     remember (dom D) as l in i. assert (ListSubset l (dom D)). { rewrite Heql. apply ListSubset_refl. } clear Heql. induction l.
     { inversion i. }
     { apply ListSubset_cons in H. destruct H as [H1 H2]. apply List.in_inv in i. destruct i.
-      { rewrite H in *. rewrite dom_spec, In_iff_exists_Some in H1. destruct H1 as (binding & mapsto). specialize (DestOnly binding mapsto). inversion DestOnly. }
+      { rewrite H in *. rewrite dom_spec, In_iff_exists_Some in H1. destruct H1 as (binding & mapsto). specialize (DestOnlyD binding mapsto). inversion DestOnlyD. }
       { specialize (IHl H H2). assumption. }
     }
 Qed.
 
-Lemma VarOnlyAtHIsNone : forall (P : ctx) (h : hvar), ctx_VarOnly P -> P (ʰ h) = None.
+Lemma VarOnlyAtHIsNone : forall (P : ctx) (h : hvar), VarOnly P -> P (ʰ h) = None.
 Proof.
-  intros * VarOnly. unfold ctx_VarOnly in VarOnly. specialize (VarOnly (ʰ h)).
+  intros * VarOnlyP. unfold VarOnly in VarOnlyP. specialize (VarOnlyP (ʰ h)).
   destruct (List.In_dec name_eq_dec (ʰ h) (dom P)).
     2:{ rewrite dom_spec in n. rewrite nIn_iff_nMapsTo in n. assumption. }
     remember (dom P) as l in i. assert (ListSubset l (dom P)). { rewrite Heql. apply ListSubset_refl. } clear Heql. induction l.
     { inversion i. }
     { apply ListSubset_cons in H. destruct H as [H1 H2]. apply List.in_inv in i. destruct i.
-      { rewrite H in *. rewrite dom_spec, In_iff_exists_Some in H1. destruct H1 as (binding & mapsto). specialize (VarOnly binding mapsto). inversion VarOnly. }
+      { rewrite H in *. rewrite dom_spec, In_iff_exists_Some in H1. destruct H1 as (binding & mapsto). specialize (VarOnlyP binding mapsto). inversion VarOnlyP. }
       { specialize (IHl H H2). assumption. }
     }
 Qed.
 
-Lemma DestOnlyUnionSingletonVarAtX : forall (D : ctx) (x : var) (m : mode) (T : type), ctx_DestOnly D -> (D ᴳ+ ᴳ{ x : m ‗ T}) (ˣ x) = Some (ₓ m ‗ T).
+Lemma DestOnlyUnionSingletonVarAtX : forall (D : ctx) (x : var) (m : mode) (T : type), DestOnly D -> (D ᴳ+ ᴳ{ x : m ‗ T}) (ˣ x) = Some (ₓ m ‗ T).
 Proof.
-  intros * DestOnly.
+  intros * DestOnlyD.
   unfold ctx_union. apply merge_with_None_Some_eq with (f := D). split.
   + apply DestOnlyAtXIsNone. assumption.
   + apply singleton_MapsKeyTo.
 Qed.
 
-Lemma IsSubtypeLinNuIsLinNu : forall (m : mode), mode_IsSubtype (¹ν) m <-> m = ¹ν.
+Lemma IsSubtypeLinNuIsLinNu : forall (m : mode), ModeSubtype (¹ν) m <-> m = ¹ν.
 Proof.
   intros m. split.
   - intros H. inversion H. inversion H2. inversion H4. reflexivity.
@@ -1493,7 +1468,7 @@ Ltac hauto_ctx :=
         DisjointHvarShiftEq,
         UnionHvarShiftEq,
         StimesHvarShiftEq,
-        hvars_max_hvars_Disjoint,
+        hvars_max_HDisjoint,
         hvarsFullShiftEq,
         MinusHvarShiftEq,
         InvMinusHvarShiftEq,
@@ -1551,7 +1526,7 @@ Ltac hauto_ctx :=
         DisjointCommutative,
         EmptyIsLinOnly,
         EmptyIsFinAgeOnly,
-        Emptybinding_IsDestOnly,
+        EmptyIsDestOnly,
         EmptyIsDisjointLeft,
         EmptyIsDisjointRight,
         EmptyIsDisposableOnly,
@@ -1588,13 +1563,13 @@ Ltac hauto_ctx :=
         hvarsMinusEq,
         hvarsInvMinusEq,
         hvars_CWkhvars_G,
-        hvars_DisjointToDisjoint,
-        DisjointTohvars_Disjoint,
+        HDisjointToDisjoint,
+        DisjointToHDisjoint,
         (* not_lt_le, *)
         HmaxSubset,
         hvarsEmpty,
-        EmptyIshvars_DisjointRight,
-        EmptyIshvars_DisjointLeft,
+        EmptyIsHDisjointRight,
+        EmptyIsHDisjointLeft,
         IsSubtype_refl,
         (* CompatibleDestSingleton,
         IncompatibleVarDestOnly, *)
@@ -1622,17 +1597,17 @@ Ltac hauto_ctx :=
         DestOnlyAtXIsNone,
         DestOnlyUnionSingletonVarAtX,
         IsSubtypeLinNuIsLinNu,
-        (* ctx_CompatibleVar_DestOnlyUnionSingleton, *)
-        (mode_IsLinProof (Fin 0)),
-        (mode_IsLinProof (Fin 1)),
-        (mode_IsFinAgeProof Lin 0),
-        (mode_IsFinAgeProof Lin 1),
-        (mode_IsValidProof (Lin, (Fin 0))),
-        (mode_IsValidProof (Lin, (Fin 1)))
+        (* CompatibleVar_DestOnlyUnionSingleton, *)
+        (IsLinProof (Fin 0)),
+        (IsLinProof (Fin 1)),
+        (IsFinAgeProof Lin 0),
+        (IsFinAgeProof Lin 1),
+        (IsValidProof (Lin, (Fin 0))),
+        (IsValidProof (Lin, (Fin 1)))
     .
 
 Ltac term_Val_no_dispose D :=
-  assert (ctx_DisposableOnly ᴳ{}) as DisposEmpty by (exact EmptyIsDisposableOnly); rewrite UnionIdentityLeft with (G := D); apply Ty_term_Val with (P := ᴳ{}); trivial.
+  assert (DisposableOnly ᴳ{}) as DisposEmpty by (exact EmptyIsDisposableOnly); rewrite UnionIdentityLeft with (G := D); apply Ty_term_Val with (P := ᴳ{}); trivial.
 
 (* Silly stuff to avoid matching hypotheses many times *)
 Definition Blocked (P : Prop) : Prop := P.
@@ -1675,27 +1650,27 @@ Ltac crush :=
     [ trivial
     | autorewrite with canonalize in *; workhorse ].
 
-Lemma TyR_val_NoVarG : forall (G : ctx) (v : val) (T : type) (TyR: G ⫦ v : T), ctx_NoVar G.
+Lemma TyR_val_NoVar : forall (G : ctx) (v : val) (T : type) (TyR: G ⫦ v : T), NoVar G.
 Proof.
-  intros * TyR. induction TyR; unfold ctx_NoVar; intros nam b mapstoG contra.
+  intros * TyR. induction TyR; unfold NoVar; intros nam b mapstoG contra.
   - unfold ctx_singleton in mapstoG. rewrite singleton_MapsTo_iff in mapstoG. apply eq_sigT_fst in mapstoG; subst. inversion contra.
   - unfold ctx_singleton in mapstoG. rewrite singleton_MapsTo_iff in mapstoG. apply eq_sigT_fst in mapstoG; subst. inversion contra.
   - unfold ctx_empty in mapstoG. simpl in mapstoG. congruence.
-  - unfold ctx_DestOnly in H. unfold ctx_NoVar in contra. specialize (H nam b mapstoG). destruct nam. { inversion H. } { inversion contra. }
-  - unfold ctx_NoVar in IHTyR. specialize (IHTyR nam b mapstoG). congruence.
-  - unfold ctx_NoVar in IHTyR. specialize (IHTyR nam b mapstoG). congruence.
+  - unfold DestOnly in H. unfold NoVar in contra. specialize (H nam b mapstoG). destruct nam. { inversion H. } { inversion contra. }
+  - unfold NoVar in IHTyR. specialize (IHTyR nam b mapstoG). congruence.
+  - unfold NoVar in IHTyR. specialize (IHTyR nam b mapstoG). congruence.
   - assert (In nam (G1 ᴳ+ G2)). { apply In_iff_exists_Some; exists b; tauto. }
     apply In_merge_iff in H. destruct H.
-    + destruct H. unfold ctx_NoVar in IHTyR1. specialize (IHTyR1 nam x H). unfold binding_IsVar in IHTyR1. destruct nam. specialize (IHTyR1 I); assumption. inversion contra.
-    + destruct H. unfold ctx_NoVar in IHTyR2. specialize (IHTyR2 nam x H). unfold binding_IsVar in IHTyR2. destruct nam. specialize (IHTyR2 I); assumption. inversion contra.
+    + destruct H. unfold NoVar in IHTyR1. specialize (IHTyR1 nam x H). unfold IsVar in IHTyR1. destruct nam. specialize (IHTyR1 I); assumption. inversion contra.
+    + destruct H. unfold NoVar in IHTyR2. specialize (IHTyR2 nam x H). unfold IsVar in IHTyR2. destruct nam. specialize (IHTyR2 I); assumption. inversion contra.
   - apply map_MapsTo_iff in mapstoG. destruct mapstoG. destruct H.
-    unfold ctx_NoVar in IHTyR. specialize (IHTyR nam x H). unfold binding_IsVar in IHTyR. destruct nam. specialize (IHTyR I); assumption. inversion contra.
+    unfold NoVar in IHTyR. specialize (IHTyR nam x H). unfold IsVar in IHTyR. destruct nam. specialize (IHTyR I); assumption. inversion contra.
   - assert (In nam (D1 ᴳ+ D2)). { apply In_iff_exists_Some; exists b; tauto. }
     apply In_merge_iff in H. destruct H.
     + assert (In nam (¹↑ ᴳ· D1 ᴳ+ D3)). { apply In_iff_exists_Some. apply In_merge_iff. left. apply In_map_iff. assumption. }
-      destruct H0. unfold ctx_NoVar in IHTyR1. specialize (IHTyR1 nam x H0). unfold binding_IsVar in IHTyR1. destruct nam. specialize (IHTyR1 I); assumption. inversion contra.
+      destruct H0. unfold NoVar in IHTyR1. specialize (IHTyR1 nam x H0). unfold IsVar in IHTyR1. destruct nam. specialize (IHTyR1 I); assumption. inversion contra.
     + assert (In nam (D2 ᴳ+ (ᴳ- D3))). { apply In_iff_exists_Some. apply In_merge_iff. left. assumption. }
-      destruct H0. unfold ctx_NoVar in IHTyR2. specialize (IHTyR2 nam x H0). unfold binding_IsVar in IHTyR2. destruct nam. specialize (IHTyR2 I); assumption. inversion contra.
+      destruct H0. unfold NoVar in IHTyR2. specialize (IHTyR2 nam x H0). unfold IsVar in IHTyR2. destruct nam. specialize (IHTyR2 I); assumption. inversion contra.
 Qed.
 
 Lemma exists_impl_to_forall : forall (A : Type) (H1 : A -> Prop) (H2 : Prop),
@@ -1708,27 +1683,27 @@ Proof.
     apply H_n. (* Applying H1 n -> H2 *)
 Qed.
 
-Lemma TyR_val_DestOnlyValHole : forall (D : ctx) (h : hvar) (T : type), (D ⫦ ᵛ- h : T) -> ctx_DestOnly D -> False.
+Lemma TyR_val_DestOnlyValHole : forall (D : ctx) (h : hvar) (T : type), (D ⫦ ᵛ- h : T) -> DestOnly D -> False.
 Proof.
   intros D h T TyRv DestOnlyD. inversion TyRv; subst.
-  specialize (DestOnlyD (ʰ h)). unfold ctx_DestOnly, ctx_singleton in DestOnlyD. specialize (DestOnlyD (₋ T ‗ ¹ν)). rewrite singleton_MapsTo_iff in DestOnlyD. sfirstorder.
+  specialize (DestOnlyD (ʰ h)). unfold DestOnly, ctx_singleton in DestOnlyD. specialize (DestOnlyD (₋ T ‗ ¹ν)). rewrite singleton_MapsTo_iff in DestOnlyD. sfirstorder.
 Qed.
 
-Lemma Ty_ectxs_DestOnlyD : forall (D : ctx) (C : ectxs) (T U0 : type) (TyC: D ⊣ C : T ↣ U0), ctx_DestOnly D.
+Lemma Ty_ectxs_DestOnlyD : forall (D : ctx) (C : ectxs) (T U0 : type) (TyC: D ⊣ C : T ↣ U0), DestOnly D.
 Proof.
   intros * TyC. induction TyC.
   all: crush.
 Qed.
 
-Lemma Ty_ectxs_hvars_Disjoint : forall (C : ectxs) (D D' : ctx) (T U0 : type) (TyC : D ⊣ C : T ↣ U0), hvars©(C) ## hvarsᴳ(D') -> D # D'.
+Lemma Ty_ectxs_HDisjoint : forall (C : ectxs) (D D' : ctx) (T U0 : type) (TyC : D ⊣ C : T ↣ U0), hvars©(C) ## hvarsᴳ(D') -> D # D'.
 Proof.
   intros * TyC hvarsDisjoint. pose proof TyC as TyC'.
   apply hvars_CWkhvars_G in TyC.
   assert (hvarsᴳ(D) ## hvarsᴳ( D')). { apply SubsetDisjoint with (H2 := hvars©(C)); assumption. }
-  apply hvars_DisjointToDisjoint in H. assumption. apply Ty_ectxs_DestOnlyD in TyC'. assumption.
+  apply HDisjointToDisjoint in H. assumption. apply Ty_ectxs_DestOnlyD in TyC'. assumption.
 Qed.
 
-Lemma Ty_ectxs_LinFinOnlyD : forall (D : ctx) (C : ectxs) (T U0 : type) (TyC: D ⊣ C : T ↣ U0), ctx_LinOnly D /\ ctx_FinAgeOnly D.
+Lemma Ty_ectxs_LinFinOnlyD : forall (D : ctx) (C : ectxs) (T U0 : type) (TyC: D ⊣ C : T ↣ U0), LinOnly D /\ FinAgeOnly D.
 Proof.
   intros D C T U0 H. induction H.
   - split. apply EmptyIsLinOnly. apply EmptyIsFinAgeOnly.
@@ -1749,12 +1724,12 @@ Proof.
   - hauto lq: on use: LinOnlyUnionEquiv, LinOnlyStimesBackward, FinAgeOnlyUnionBackward, FinAgeOnlyStimesBackward, LinOnlyWkValidOnly.
   - hauto lq: on use: LinOnlyUnionEquiv, LinOnlyStimesBackward, FinAgeOnlyUnionBackward, FinAgeOnlyStimesBackward, LinOnlyWkValidOnly.
   - hauto lq: on use: LinOnlyUnionEquiv, LinOnlyStimesBackward, FinAgeOnlyUnionBackward, FinAgeOnlyStimesBackward, LinOnlyWkValidOnly.
-  - assert (ctx_LinOnly (¹↑ ᴳ· D1)).
-      { hauto use: LinOnlyUnionEquiv, LinOnlyStimesForward, (mode_IsLinProof (Fin 1)). }
-    assert (ctx_FinAgeOnly (¹↑ ᴳ· D1)).
-      { hauto use: FinAgeOnlyUnionBackward, FinAgeOnlyStimesForward, (mode_IsFinAgeProof Lin 1). }
+  - assert (LinOnly (¹↑ ᴳ· D1)).
+      { hauto use: LinOnlyUnionEquiv, LinOnlyStimesForward, (IsLinProof (Fin 1)). }
+    assert (FinAgeOnly (¹↑ ᴳ· D1)).
+      { hauto use: FinAgeOnlyUnionBackward, FinAgeOnlyStimesForward, (IsFinAgeProof Lin 1). }
     assert ((D1 ᴳ+ D2) # (ᴳ- D3)).
-      { apply (Ty_ectxs_hvars_Disjoint C (D1 ᴳ+ D2) (ᴳ- D3) (U ⧔ T') U0); tauto. }
+      { apply (Ty_ectxs_HDisjoint C (D1 ᴳ+ D2) (ᴳ- D3) (U ⧔ T') U0); tauto. }
     assert ((¹↑ ᴳ· D1) # D3).
       { sblast use: DisjointNestedLeftEquiv, DisjointMinusRightEquiv, DisjointStimesLeftEquiv. }
     rewrite LinOnlyUnionEquiv. repeat split. tauto. tauto. tauto. apply FinAgeOnlyUnionForward. repeat split. all:tauto.
@@ -1767,14 +1742,14 @@ Proof.
   - right. exists n. rewrite <- In_iff_exists_Some. apply dom_spec. rewrite eDomG. apply List.in_eq.
 Qed.
 
-Lemma LinOnlyWithStimes_dec : forall (D1 D2 : ctx) (m' : mode), mode_IsValid m' -> ctx_LinOnly (m' ᴳ· D1 ᴳ+ D2) -> { mode_IsLin m' } + { mode_IsUr m' /\ D1 = ᴳ{} }.
+Lemma LinOnlyWithStimes_dec : forall (D1 D2 : ctx) (m' : mode), IsValid m' -> LinOnly (m' ᴳ· D1 ᴳ+ D2) -> { IsLin m' } + { IsUr m' /\ D1 = ᴳ{} }.
 Proof.
   intros * Validmp LinOnlyD.
-  destruct (mode_IsLin_dec m'). { left. assumption. }
-  right. assert (mode_IsUr m'). { destruct m'. destruct p. destruct m. specialize (n (mode_IsLinProof a)). contradiction. constructor. inversion Validmp. }
+  destruct (IsLin_dec m'). { left. assumption. }
+  right. assert (IsUr m'). { destruct m'. destruct p. destruct m. specialize (n (IsLinProof a)). contradiction. constructor. inversion Validmp. }
   split. assumption.
   apply ext_eq. rename n into NotLin. intros n.
-    assert (ctx_LinOnly (m' ᴳ· D1)). { crush. } unfold ctx_LinOnly in H0. destruct (Empty_dec D1).
+    assert (LinOnly (m' ᴳ· D1)). { crush. } unfold LinOnly in H0. destruct (Empty_dec D1).
     - rewrite e. cbn. reflexivity.
     - destruct e as (n' & mapstoD1). exfalso.
       unfold ctx_stimes in H0. specialize (H0 n').
@@ -1788,10 +1763,10 @@ end)) in inD1. rewrite In_iff_exists_Some in inD1. destruct inD1 as (binding & m
 Qed.
 
 Lemma SplitDestOnlyVarOnly : forall (P1 P2 D1 D2 : ctx),
-  ctx_VarOnly P1 ->
-  ctx_VarOnly P2 ->
-  ctx_DestOnly D1 ->
-  ctx_DestOnly D2 ->
+  VarOnly P1 ->
+  VarOnly P2 ->
+  DestOnly D1 ->
+  DestOnly D2 ->
   (P1 ᴳ+ D1 = P2 ᴳ+ D2) ->
   (P1 = P2 /\ D1 = D2).
 Proof.
@@ -1807,10 +1782,10 @@ Qed.
 
 Lemma TermSubLemma :
   forall (D1 D2 : ctx) (m' : mode) (T' U' : type) (te : term) (x' : var) (v' : val),
-  mode_IsValid m' ->
-  ctx_DestOnly D1 ->
-  ctx_DestOnly D2 ->
-  ctx_LinOnly (m' ᴳ· D1 ᴳ+ D2) ->
+  IsValid m' ->
+  DestOnly D1 ->
+  DestOnly D2 ->
+  LinOnly (m' ᴳ· D1 ᴳ+ D2) ->
   (D2 ᴳ+ ᴳ{ x' : m' ‗ T'} ⊢ te : U') ->
   (D1 ⊢ ᵥ₎ v' : T') ->
   (m' ᴳ· D1 ᴳ+ D2 ⊢ te ᵗ[ x' ≔ v'] : U').
@@ -1826,8 +1801,8 @@ Proof.
       } destruct UnionEqSplit; subst.
     assert (ᴳ{ x' : m' ‗ T'} (ˣ x') = Some (ₓ m' ‗ T')) as mapstoSing.
       { unfold ctx_singleton. apply (@singleton_MapsKeyTo name binding_type_of). }
-    assert (mode_IsUr m'). { unfold ctx_DisposableOnly in DisposP. specialize (DisposP (ˣ x') (ₓ m' ‗ T') mapstoSing). simpl in DisposP. assumption. }
-    assert (D1 = ᴳ{}). { destruct (LinOnlyWithStimes_dec D1 D2 m' Validmp LinOnlyD). inversion H0. inversion m. congruence. destruct a. assumption. }
+    assert (IsUr m'). { unfold DisposableOnly in DisposP. specialize (DisposP (ˣ x') (ₓ m' ‗ T') mapstoSing). simpl in DisposP. assumption. }
+    assert (D1 = ᴳ{}). { destruct (LinOnlyWithStimes_dec D1 D2 m' Validmp LinOnlyD). inversion H0. inversion i. congruence. destruct a. assumption. }
     rewrite H1 in *. rewrite StimesEmptyEq. rewrite <- UnionIdentityLeft. term_Val_no_dispose D2.
   - rename x into Hu, x0 into x.
     assert (P ᴳ+ (ᴳ{ x : m ‗ T}) = D2 ᴳ+ ᴳ{ x' : m' ‗ T'}) as UnionEq.
@@ -1837,11 +1812,11 @@ Admitted.
 
 Lemma TermSubLemma2 :
   forall (D11 D12 D2 : ctx) (m' : mode) (T1' T2' U' : type) (te : term) (x1' x2' : var) (v1' v2' : val),
-  mode_IsValid m' ->
-  ctx_DestOnly D11 ->
-  ctx_DestOnly D12 ->
-  ctx_DestOnly D2 ->
-  ctx_LinOnly (m' ᴳ· (D11 ᴳ+ D12) ᴳ+ D2) ->
+  IsValid m' ->
+  DestOnly D11 ->
+  DestOnly D12 ->
+  DestOnly D2 ->
+  LinOnly (m' ᴳ· (D11 ᴳ+ D12) ᴳ+ D2) ->
   (ᴳ{ x1' : m' ‗ T1'} # ᴳ{ x2' : m' ‗ T2'}) ->
   (D2 ᴳ+ ᴳ{ x1' : m' ‗ T1'} ᴳ+ ᴳ{ x2' : m' ‗ T2'} ⊢ te : U') ->
   (D11 ⊢ ᵥ₎ v1' : T1') ->
@@ -1853,12 +1828,12 @@ Lemma EctxsSubLemma : forall (D1 D2 D3: ctx) (h : hvar) (C : ectxs) (m n : mode)
   D1 # D2 ->
   D1 # D3 ->
   hvars©(C) ## hvarsᴳ(ᴳ- D3) ->
-  ctx_DestOnly D1 ->
-  ctx_DestOnly D2 ->
-  ctx_DestOnly D3 ->
-  ctx_LinOnly D3 ->
-  ctx_FinAgeOnly D3 ->
-  ctx_ValidOnly D3 ->
+  DestOnly D1 ->
+  DestOnly D2 ->
+  DestOnly D3 ->
+  LinOnly D3 ->
+  FinAgeOnly D3 ->
+  ValidOnly D3 ->
   D1 # ᴳ{+ h : m ⌊ U ⌋ n } ->
   D2 # ᴳ{+ h : m ⌊ U ⌋ n } ->
   D3 # ᴳ{+ h : m ⌊ U ⌋ n } ->
@@ -1882,7 +1857,7 @@ Proof.
     - (* Sem-eterm-AppFoc1 *)
       inversion Tyt; subst.
       rename Tyt into TyApp, Tyt0 into Tyt, P1 into D1, P2 into D2, T into U, T0 into T.
-      assert (ctx_LinOnly (m ᴳ· D1 ᴳ+ D2)) as LinOnlyD.
+      assert (LinOnly (m ᴳ· D1 ᴳ+ D2)) as LinOnlyD.
         { apply (Ty_ectxs_LinFinOnlyD (m ᴳ· D1 ᴳ+ D2) C U U0); tauto. }
       constructor 1 with (D := D1) (T := T) (t := t); swap 1 3. constructor 2 with (D2 := D2) (m := m) (t' := t') (U := U).
       all: crush.
@@ -1890,7 +1865,7 @@ Proof.
       inversion Tyt; subst. rename TyC into TyCc, D0 into D1, ValidOnlyD into ValidOnlyD1, DestOnlyD into DestOnlyD1. clear H1.
       inversion TyCc; subst. clear DestOnlyD0.
       rewrite (SimplifyDisposableInTyC P D1 DisposP DestOnlyD1) in *.
-      assert (ctx_LinOnly (m ᴳ· D1 ᴳ+ D2)) as LinOnlyD.
+      assert (LinOnly (m ᴳ· D1 ᴳ+ D2)) as LinOnlyD.
         { apply (Ty_ectxs_LinFinOnlyD (m ᴳ· D1 ᴳ+ D2) C U U0); tauto. }
       assert (m ᴳ· D1 ᴳ+ D2 ⊢ ᵥ₎ v ≻ t' : U) as TyApp.
         { apply (Ty_term_App m D1 D2 (ᵥ₎ v) t' U T); tauto. }
@@ -1899,7 +1874,7 @@ Proof.
     - (* Sem-eterm-AppFoc2 *)
       inversion Tyt; subst.
       rename Tyt into TyApp, Tyt0 into Tyt, P1 into D1, P2 into D2, T into U, T0 into T.
-      assert (ctx_LinOnly (m ᴳ· D1 ᴳ+ D2)) as LinOnlyD.
+      assert (LinOnly (m ᴳ· D1 ᴳ+ D2)) as LinOnlyD.
         { apply (Ty_ectxs_LinFinOnlyD (m ᴳ· D1 ᴳ+ D2) C U U0); tauto. }
         constructor 1 with (D := D2) (T := T ⁔ m → U) (t := t'); swap 1 3. constructor 3 with (D1 := D1) (m := m) (v := v) (T := T) (U := U).
       all: crush.
@@ -1909,7 +1884,7 @@ Proof.
       rewrite (SimplifyDisposableInTyC P D2 DisposP DestOnlyD2) in *.
       assert (m ᴳ· D1 ᴳ+ D2 ⊢ ᵥ₎ v ≻ ᵥ₎ v' : U) as TyApp.
         { apply (Ty_term_App m D1 D2 (ᵥ₎ v) (ᵥ₎ v') U T); tauto. }
-      assert (ctx_LinOnly (m ᴳ· D1 ᴳ+ D2)) as LinOnlyD.
+      assert (LinOnly (m ᴳ· D1 ᴳ+ D2)) as LinOnlyD.
         { apply (Ty_ectxs_LinFinOnlyD (m ᴳ· D1 ᴳ+ D2) C U U0); tauto. }
       constructor 1 with (D := (m ᴳ· D1 ᴳ+ D2)) (T := U) (t := (ᵥ₎ v) ≻ (ᵥ₎ v')).
       all: crush.
@@ -1919,10 +1894,10 @@ Proof.
         { inversion_clear Tytp; inversion_clear TyRv; tauto. }
       rewrite <- Eqmm0 in *. clear Eqmm0. clear m0. rename P1 into D1, P2 into D2. rename Tyt into TyApp, Tyt0 into Tyt, T into U, T0 into T.
       inversion Tytp; subst. clear H1. rename TyRv into TyRv', D into D2.
-      assert (ctx_DestOnly (P ᴳ+ D2)) as DestOnlyPuD2. { crush. }
+      assert (DestOnly (P ᴳ+ D2)) as DestOnlyPuD2. { crush. }
       rewrite (SimplifyDisposableInTyC P D2 DisposP DestOnlyPuD2) in *.
       inversion TyRv'; subst. rename H1 into DestOnlyD2.
-      assert (ctx_LinOnly (m ᴳ· D1 ᴳ+ D2)) as LinOnlyD.
+      assert (LinOnly (m ᴳ· D1 ᴳ+ D2)) as LinOnlyD.
         { apply (Ty_ectxs_LinFinOnlyD (m ᴳ· D1 ᴳ+ D2) C U U0); tauto. }
       assert (m ᴳ· D1 ᴳ+ D2 ⊢ u ᵗ[ x ≔ v] : U) as Tyusub.
       { apply (TermSubLemma D1 D2 m T U u x v). all: crush. }
@@ -1931,14 +1906,14 @@ Proof.
     - (* Sem-eterm-PatUFoc *)
       inversion Tyt; subst.
       rename Tyt into TyPat, Tyt0 into Tyt, P1 into D1, P2 into D2, T into T2.
-      assert (ctx_LinOnly (D1 ᴳ+ D2)) as LinOnlyD.
+      assert (LinOnly (D1 ᴳ+ D2)) as LinOnlyD.
         { apply (Ty_ectxs_LinFinOnlyD (D1 ᴳ+ D2) C T2 U0); tauto. }
         constructor 1 with (D := D1) (T := ①) (t := t); swap 1 3. constructor 4 with (D2 := D2) (U := T2) (u := u). all: crush.
     - (* Sem-eterm-PatUUnfoc *)
       inversion Tyt; subst. rename TyC into TyCc, D0 into D1, ValidOnlyD into ValidOnlyD1, DestOnlyD into DestOnlyD1. clear H1.
       inversion TyCc; subst. clear DestOnlyD0. rename U into T2.
       rewrite (SimplifyDisposableInTyC P D1 DisposP DestOnlyD1) in *.
-      assert (ctx_LinOnly (D1 ᴳ+ D2)) as LinOnlyD.
+      assert (LinOnly (D1 ᴳ+ D2)) as LinOnlyD.
         { apply (Ty_ectxs_LinFinOnlyD (D1 ᴳ+ D2) C T2 U0); tauto. }
       assert (D1 ᴳ+ D2 ⊢ ᵥ₎ v ᵗ; u : T2) as TyPat.
         { apply (Ty_term_PatU D1 D2 (ᵥ₎ v) u T2); tauto. }
@@ -1952,14 +1927,14 @@ Proof.
     - (* Sem-eterm-PatSFoc *)
       inversion Tyt; subst.
       rename Tyt into TyPat, Tyt0 into Tyt, P1 into D1, P2 into D2, T into U.
-      assert (ctx_LinOnly (m ᴳ· D1 ᴳ+ D2)) as LinOnlyD.
+      assert (LinOnly (m ᴳ· D1 ᴳ+ D2)) as LinOnlyD.
         { apply (Ty_ectxs_LinFinOnlyD (m ᴳ· D1 ᴳ+ D2) C U U0); tauto. }
       constructor 1 with (D := D1) (T := (T1 ⨁ T2)) (t := t) ; swap 1 3. constructor 5 with (D1 := D1) (D2 := D2) (m := m) (u1 := u1) (x1 := x1) (u2 := u2) (x2 := x2) (U := U). all: crush.
     - (* Sem-eterm-PatSUnfoc *)
       inversion Tyt; subst. rename TyC into TyCc, D0 into D1, ValidOnlyD into ValidOnlyD1, DestOnlyD into DestOnlyD1. clear H1.
       inversion TyCc; subst. clear DestOnlyD0.
       rewrite (SimplifyDisposableInTyC P D1 DisposP DestOnlyD1) in *.
-      assert (ctx_LinOnly (m ᴳ· D1 ᴳ+ D2)) as LinOnlyD.
+      assert (LinOnly (m ᴳ· D1 ᴳ+ D2)) as LinOnlyD.
         { apply (Ty_ectxs_LinFinOnlyD (m ᴳ· D1 ᴳ+ D2) C U U0); tauto. }
       assert (m ᴳ· D1 ᴳ+ D2 ⊢ ᵥ₎ v ≻caseˢ m {Inl x1 ⟼ u1, Inr x2 ⟼ u2} : U) as TyPat.
         { apply (Ty_term_PatS m D1 D2 (ᵥ₎ v) x1 u1 x2 u2 U T1 T2); crush. }
@@ -1969,11 +1944,11 @@ Proof.
       rename P1 into D1, P2 into D2. rename Tyt into TyPat, Tyt0 into Tyt, T into U.
       inversion Tyt; subst. rename H1 into DestOnlyD1, TyRv into TyRInlv1, D into D1.
       inversion TyRInlv1; subst.
-      assert (ctx_DestOnly (P ᴳ+ D1)) as DestOnlyPuD1. { crush. }
+      assert (DestOnly (P ᴳ+ D1)) as DestOnlyPuD1. { crush. }
       rewrite (SimplifyDisposableInTyC P D1 DisposP DestOnlyPuD1) in *.
       assert (D1 ⊢ ᵥ₎ v1 : T1) as Tyt'.
         { term_Val_no_dispose D1. }
-      assert (ctx_LinOnly (m ᴳ· D1 ᴳ+ D2)) as LinOnlyD.
+      assert (LinOnly (m ᴳ· D1 ᴳ+ D2)) as LinOnlyD.
         { apply (Ty_ectxs_LinFinOnlyD (m ᴳ· D1 ᴳ+ D2) C U U0); tauto. }
       assert (m ᴳ· D1 ᴳ+ D2 ⊢ u1 ᵗ[ x1 ≔ v1] : U) as Tyusub.
         { apply (TermSubLemma D1 D2 m T1 U u1 x1 v1); crush. }
@@ -1983,11 +1958,11 @@ Proof.
       rename P1 into D1, P2 into D2. rename Tyt into TyPat, Tyt0 into Tyt, T into U.
       inversion Tyt; subst. rename H1 into DestOnlyD1, TyRv into TyRInlv2, D into D1.
       inversion TyRInlv2; subst.
-      assert (ctx_DestOnly (P ᴳ+ D1)) as DestOnlyPuD1. { crush. }
+      assert (DestOnly (P ᴳ+ D1)) as DestOnlyPuD1. { crush. }
       rewrite (SimplifyDisposableInTyC P D1 DisposP DestOnlyPuD1) in *.
       assert (D1 ⊢ ᵥ₎ v2 : T2) as Tyt'.
         { term_Val_no_dispose D1. }
-      assert (ctx_LinOnly (m ᴳ· D1 ᴳ+ D2)) as LinOnlyD.
+      assert (LinOnly (m ᴳ· D1 ᴳ+ D2)) as LinOnlyD.
         { apply (Ty_ectxs_LinFinOnlyD (m ᴳ· D1 ᴳ+ D2) C U U0); tauto. }
       assert (m ᴳ· D1 ᴳ+ D2 ⊢ u2 ᵗ[ x2 ≔ v2] : U) as Tyusub.
         { apply (TermSubLemma D1 D2 m T2 U u2 x2 v2); crush. }
@@ -1995,14 +1970,14 @@ Proof.
     - (* Sem-eterm-PatPFoc *)
       inversion Tyt; subst.
       rename Tyt into TyPat, Tyt0 into Tyt, P1 into D1, P2 into D2, T into U.
-      assert (ctx_LinOnly (m ᴳ· D1 ᴳ+ D2)) as LinOnlyD.
+      assert (LinOnly (m ᴳ· D1 ᴳ+ D2)) as LinOnlyD.
         { apply (Ty_ectxs_LinFinOnlyD (m ᴳ· D1 ᴳ+ D2) C U U0); tauto. }
       constructor 1 with (D := D1) (T := (T1 ⨂ T2)) (t := t) ; swap 1 3. constructor 6 with (D1 := D1) (D2 := D2) (u := u) (x1 := x1) (x2 := x2) (U := U). all: crush.
     - (* Sem-eterm-PatPUnfoc *)
       inversion Tyt; subst. rename TyC into TyCc, D0 into D1, ValidOnlyD into ValidOnlyD1, DestOnlyD into DestOnlyD1. clear H1.
       inversion TyCc; subst. clear DestOnlyD0.
       rewrite (SimplifyDisposableInTyC P D1 DisposP DestOnlyD1) in *.
-      assert (ctx_LinOnly (m ᴳ· D1 ᴳ+ D2)) as LinOnlyD.
+      assert (LinOnly (m ᴳ· D1 ᴳ+ D2)) as LinOnlyD.
         { apply (Ty_ectxs_LinFinOnlyD (m ᴳ· D1 ᴳ+ D2) C U U0); tauto. }
       assert (m ᴳ· D1 ᴳ+ D2 ⊢ ᵥ₎ v ≻caseᵖ m ᵗ(x1 , x2) ⟼ u : U) as TyPat.
         { apply (Ty_term_PatP m D1 D2 (ᵥ₎ v) x1 x2 u U T1 T2); crush. }
@@ -2012,13 +1987,13 @@ Proof.
       rename P1 into D1, P2 into D2. rename Tyt into TyPat, Tyt0 into Tyt, T into U.
       inversion Tyt; subst. rename H1 into DestOnlyD1, D into D1.
       inversion TyRv; subst. rename G1 into D11, G2 into D12.
-      assert (ctx_DestOnly (P ᴳ+ (D11 ᴳ+ D12))) as DestOnlyPuD1. { crush. }
+      assert (DestOnly (P ᴳ+ (D11 ᴳ+ D12))) as DestOnlyPuD1. { crush. }
       rewrite (SimplifyDisposableInTyC P (D11 ᴳ+ D12) DisposP DestOnlyPuD1) in *.
       assert (D11 ⊢ ᵥ₎ v1 : T1) as Tyt1.
         { term_Val_no_dispose D11. crush. }
       assert (D12 ⊢ ᵥ₎ v2 : T2) as Tyt2.
         { term_Val_no_dispose D12. crush. }
-      assert (ctx_LinOnly (m ᴳ· (D11 ᴳ+ D12) ᴳ+ D2)) as LinOnlyD.
+      assert (LinOnly (m ᴳ· (D11 ᴳ+ D12) ᴳ+ D2)) as LinOnlyD.
         { apply (Ty_ectxs_LinFinOnlyD (m ᴳ· (D11 ᴳ+ D12) ᴳ+ D2) C U U0); tauto. }
       assert (m ᴳ· (D11 ᴳ+ D12) ᴳ+ D2 ⊢ u ᵗ[ x1 ≔ v1] ᵗ[ x2 ≔ v2] : U) as Tyusub.
         { apply (TermSubLemma2 D11 D12 D2 m T1 T2 U u x1 x2 v1 v2); crush. }
@@ -2026,14 +2001,14 @@ Proof.
     - (* Sem-eterm-PatEFoc *)
       inversion Tyt; subst.
       rename Tyt into TyPat, Tyt0 into Tyt, P1 into D1, P2 into D2, T into U, T0 into T.
-      assert (ctx_LinOnly (m ᴳ· D1 ᴳ+ D2)) as LinOnlyD.
+      assert (LinOnly (m ᴳ· D1 ᴳ+ D2)) as LinOnlyD.
         { apply (Ty_ectxs_LinFinOnlyD (m ᴳ· D1 ᴳ+ D2) C U U0); tauto. }
       constructor 1 with (D := D1) (T := (! n ⁔ T)) (t := t) ; swap 1 3. constructor 7 with (D1 := D1) (D2 := D2) (u := u) (x := x) (U := U). all: crush.
     - (* Sem-eterm-PatEUnfoc *)
       inversion Tyt; subst. rename TyC into TyCc, D0 into D1, ValidOnlyD into ValidOnlyD1, DestOnlyD into DestOnlyD1. clear H1.
       inversion TyCc; subst. clear DestOnlyD0. rename T0 into T.
       rewrite (SimplifyDisposableInTyC P D1 DisposP DestOnlyD1) in *.
-      assert (ctx_LinOnly (m ᴳ· D1 ᴳ+ D2)) as LinOnlyD.
+      assert (LinOnly (m ᴳ· D1 ᴳ+ D2)) as LinOnlyD.
         { apply (Ty_ectxs_LinFinOnlyD (m ᴳ· D1 ᴳ+ D2) C U U0); tauto. }
       assert (m ᴳ· D1 ᴳ+ D2 ⊢ ᵥ₎ v ≻caseᵉ m ᴇ n ⁔ x ⟼ u : U) as TyPat.
         { apply (Ty_term_PatE m D1 D2 (ᵥ₎ v) n x u U T); crush. }
@@ -2043,11 +2018,11 @@ Proof.
       rename P1 into D1, P2 into D2. rename Tyt into TyPat, Tyt0 into Tyt, T into U, T0 into T.
       inversion Tyt; subst. rename H1 into DestOnlyD1.
       inversion TyRv; subst. rename G into D1.
-      assert (ctx_DestOnly (P ᴳ+ (n ᴳ· D1))) as DestOnlyPuD1. { crush. }
+      assert (DestOnly (P ᴳ+ (n ᴳ· D1))) as DestOnlyPuD1. { crush. }
       rewrite (SimplifyDisposableInTyC P (n ᴳ· D1) DisposP DestOnlyPuD1) in *.
       assert (D1 ⊢ ᵥ₎ v' : T) as Tyt'.
         { term_Val_no_dispose D1. crush. }
-      assert (ctx_LinOnly (m ᴳ· (n ᴳ· D1) ᴳ+ D2)) as LinOnlyD.
+      assert (LinOnly (m ᴳ· (n ᴳ· D1) ᴳ+ D2)) as LinOnlyD.
         { apply (Ty_ectxs_LinFinOnlyD (m ᴳ· (n ᴳ· D1) ᴳ+ D2) C U U0); tauto. }
       assert ((m · n) ᴳ· D1 ᴳ+ D2 ⊢ u ᵗ[ x ≔ v'] : U) as Tyusub.
         { apply (TermSubLemma D1 D2 (m · n) T U u x v'). all: crush. }
@@ -2055,14 +2030,14 @@ Proof.
     - (* Sem-eterm-MapFoc *)
       inversion Tyt; subst. rename T0 into T.
       rename Tyt into TyMap, Tyt0 into Tyt, P1 into D1, P2 into D2.
-      assert (ctx_LinOnly (D1 ᴳ+ D2)) as LinOnlyD.
+      assert (LinOnly (D1 ᴳ+ D2)) as LinOnlyD.
         { apply (Ty_ectxs_LinFinOnlyD (D1 ᴳ+ D2) C (U ⧔ T') U0); tauto. }
       constructor 1 with (D := D1) (T := U ⧔ T) (t := t); swap 1 3. constructor 8 with (D1 := D1) (D2 := D2) (t' := t') (x := x) (T := T) (T' := T') (U := U). all: crush.
     - (* Sem-eterm-MapUnfoc *)
       inversion Tyt; subst. rename TyC into TyCc, D0 into D1, ValidOnlyD into ValidOnlyD1, DestOnlyD into DestOnlyD1. clear H1.
       inversion TyCc; subst. clear DestOnlyD0. rename T0 into T.
       rewrite (SimplifyDisposableInTyC P D1 DisposP DestOnlyD1) in *.
-      assert (ctx_LinOnly (D1 ᴳ+ D2)) as LinOnlyD.
+      assert (LinOnly (D1 ᴳ+ D2)) as LinOnlyD.
         { apply (Ty_ectxs_LinFinOnlyD (D1 ᴳ+ D2) C (U ⧔ T') U0); tauto. }
       assert (D1 ᴳ+ D2 ⊢ ᵥ₎ v ≻map x ⟼ t' : U ⧔ T') as TyMap.
         { apply (Ty_term_Map D1 D2 (ᵥ₎ v) x t' U T' T); crush. }
@@ -2072,7 +2047,7 @@ Proof.
       rename P1 into D1, P2 into D2. rename Tyt into TyMap, Tyt0 into Tyt, T0 into T.
       inversion Tyt; subst. rename H2 into DestOnlyD1.
       inversion TyRv; subst. rename D1 into D11, D0 into D12, D3 into D13, DestOnlyD0 into DestOnlyD11, DestOnlyD2 into DestOnlyD12, DestOnlyD3 into DestOnlyD13, LinOnlyD3 into LinOnlyD13, ValidOnlyD3 into ValidOnlyD13, DisjointD1D2 into DisjointD11D12, DisjointD1D3 into DisjointD11D13, DisjointD2D3 into DisjointD12D13, FinAgeOnlyD3 into FinAgeOnlyD13.
-      assert (ctx_DestOnly (P ᴳ+ (D11 ᴳ+ D12))) as DestOnlyPuD1. { crush. }
+      assert (DestOnly (P ᴳ+ (D11 ᴳ+ D12))) as DestOnlyPuD1. { crush. }
       rewrite (SimplifyDisposableInTyC P (D11 ᴳ+ D12) DisposP DestOnlyPuD1) in *.
       assert ((D2 ᴳ+ D11) # (D13 ᴳ[ hvarsᴳ(ᴳ- D13) ⩲ (maxᴴ(hvars©(C)) + 1)])) as DisjointD2uD11D13. {
           {  apply DisjointNestedLeftEquiv. assert (NatSet.Subset hvarsᴳ(D11 ᴳ+ D12 ᴳ+ D2) hvars©(C)).
@@ -2082,20 +2057,20 @@ Proof.
               assert (maxᴴ(hvarsᴳ(D2)) <= maxᴴ(hvars©(C))).
               { apply HmaxSubset. tauto. }
               assert (hvarsᴳ(D2) ## (hvarsᴳ(D13) ᴴ⩲ (maxᴴ(hvars©(C)) + 1))).
-              { apply hvars_max_hvars_Disjoint; rewrite Nat.add_comm; unfold lt, plus; apply le_n_S; tauto. }
+              { apply hvars_max_HDisjoint; rewrite Nat.add_comm; unfold lt, plus; apply le_n_S; tauto. }
               assert (hvarsᴳ(D2) ## hvarsᴳ( D13 ᴳ[ hvarsᴳ(ᴳ- D13) ⩲ (maxᴴ(hvars©(C)) + 1)])).
-              { unfold hvars_Disjoint. rewrite hvarsMinusEq. rewrite hvarsFullShiftEq. tauto. }
-              apply hvars_DisjointToDisjoint; crush.
+              { unfold HDisjoint. rewrite hvarsMinusEq. rewrite hvarsFullShiftEq. tauto. }
+              apply HDisjointToDisjoint; crush.
             }
             { assert (NatSet.Subset hvarsᴳ(D11) hvars©(C)).
               { apply HvarsSubsetCtxUnionBackward in H. destruct H. apply HvarsSubsetCtxUnionBackward in H. tauto. }
               assert (maxᴴ(hvarsᴳ(D11)) <= maxᴴ(hvars©(C))).
               { apply HmaxSubset. tauto. }
               assert (hvarsᴳ(D11) ## (hvarsᴳ(D13) ᴴ⩲ (maxᴴ(hvars©(C)) + 1))).
-              { apply hvars_max_hvars_Disjoint; rewrite Nat.add_comm; unfold lt, plus; apply le_n_S; tauto. }
+              { apply hvars_max_HDisjoint; rewrite Nat.add_comm; unfold lt, plus; apply le_n_S; tauto. }
               assert (hvarsᴳ(D11) ## hvarsᴳ( D13 ᴳ[ hvarsᴳ(ᴳ- D13) ⩲ (maxᴴ(hvars©(C)) + 1)])).
               { rewrite hvarsMinusEq. rewrite hvarsFullShiftEq. tauto. }
-              apply hvars_DisjointToDisjoint; crush.
+              apply HDisjointToDisjoint; crush.
             }
           } }
       assert ((¹↑ ᴳ· D11 ᴳ+ D13) ᴳ[hvarsᴳ(ᴳ- D13) ⩲ (maxᴴ(hvars©(C)) + 1)] ⊢ ᵥ₎ v1 ᵛ[hvarsᴳ(ᴳ- D13) ⩲ (maxᴴ(hvars©(C)) + 1)] : T) as Tyt1.
@@ -2106,15 +2081,15 @@ Proof.
         assert (D11 ᴳ[ hvarsᴳ(ᴳ- D13) ⩲ (maxᴴ(hvars©(C)) + 1)] = D11) as D11Eq by ( apply DisjointHvarShiftEq; crush );
         assert (D12 ᴳ[ hvarsᴳ(ᴳ- D13) ⩲ (maxᴴ(hvars©(C)) + 1)] = D12) as D12Eq by ( apply DisjointHvarShiftEq; crush );
         rewrite D11Eq.
-        { assert (ctx_ValidOnly (¹↑ ᴳ· (D2 ᴳ+ D11))).
+        { assert (ValidOnly (¹↑ ᴳ· (D2 ᴳ+ D11))).
           { apply ValidOnlyStimesForward. split.
             - rewrite (UnionCommutative (D11 ᴳ+ D12) D2) in ValidOnlyD.
               rewrite UnionAssociative in ValidOnlyD.
               apply ValidOnlyUnionBackward in ValidOnlyD.
               tauto.
-            - exact (mode_IsValidProof (Lin, Fin 1)).
+            - exact (IsValidProof (Lin, Fin 1)).
           }
-          assert (ctx_ValidOnly (D13 ᴳ[ hvarsᴳ(ᴳ- D13) ⩲ (maxᴴ(hvars©(C)) + 1)])).
+          assert (ValidOnly (D13 ᴳ[ hvarsᴳ(ᴳ- D13) ⩲ (maxᴴ(hvars©(C)) + 1)])).
           { apply ValidOnlyHvarShiftEquiv; tauto. }
 
           apply ValidOnlyUnionForward; crush.
@@ -2132,18 +2107,18 @@ Proof.
             rewrite UnionAssociative.
             rewrite StimesUnionDistributive. tauto. }
           rewrite ctxEq.
-          assert (ctx_ValidOnly ((¹↑ ᴳ· D11 ᴳ+ D13) ᴳ[ hvarsᴳ(ᴳ- D13) ⩲ (maxᴴ( hvars©( C)) + 1)])).
+          assert (ValidOnly ((¹↑ ᴳ· D11 ᴳ+ D13) ᴳ[ hvarsᴳ(ᴳ- D13) ⩲ (maxᴴ( hvars©( C)) + 1)])).
             { apply ValidOnlyHvarShiftEquiv. apply ValidOnlyUnionForward; trivial.
              { apply ValidOnlyStimesForward; split; crush. }
              { crush. }
             }
-          assert (ctx_LinOnly (D11 ᴳ+ D12 ᴳ+ D2)) as LinOnlyD.
+          assert (LinOnly (D11 ᴳ+ D12 ᴳ+ D2)) as LinOnlyD.
             { apply (Ty_ectxs_LinFinOnlyD (D11 ᴳ+ D12 ᴳ+ D2) C (U ⧔ T') U0); tauto. }
-          assert (ctx_LinOnly ((¹ν ᴳ· (¹↑ ᴳ· D11 ᴳ+ D13) ᴳ[ hvarsᴳ(ᴳ- D13) ⩲ (maxᴴ(hvars©(C)) + 1)]) ᴳ+ ¹↑ ᴳ· D2)).
+          assert (LinOnly ((¹ν ᴳ· (¹↑ ᴳ· D11 ᴳ+ D13) ᴳ[ hvarsᴳ(ᴳ- D13) ⩲ (maxᴴ(hvars©(C)) + 1)]) ᴳ+ ¹↑ ᴳ· D2)).
             { apply LinOnlyUnionEquiv; repeat split.
-              { apply LinOnlyStimesForward. exact (mode_IsLinProof (Fin 0)). apply LinOnlyHvarShiftEquiv. apply LinOnlyUnionEquiv; repeat split. apply LinOnlyStimesForward. exact (mode_IsLinProof (Fin 1)). crush.
+              { apply LinOnlyStimesForward. exact (IsLinProof (Fin 0)). apply LinOnlyHvarShiftEquiv. apply LinOnlyUnionEquiv; repeat split. apply LinOnlyStimesForward. exact (IsLinProof (Fin 1)). crush.
               assumption. crush. }
-              { apply LinOnlyStimesForward. exact (mode_IsLinProof (Fin 1)). crush. }
+              { apply LinOnlyStimesForward. exact (IsLinProof (Fin 1)). crush. }
               { apply DisjointStimesLeftEquiv. rewrite UnionHvarShiftEq. apply DisjointNestedLeftEquiv. split. rewrite StimesHvarShiftEq. rewrite DisjointHvarShiftEq. rewrite DisjointStimesLeftEquiv, DisjointStimesRightEquiv. crush. crush. apply DisjointCommutative. rewrite StimesUnionDistributive, DisjointNestedLeftEquiv in H. destruct H as (H & H'). assumption. }
             }
           apply TermSubLemma with (T' := T) (D2 := ¹↑ ᴳ· D2).
@@ -2151,9 +2126,9 @@ Proof.
         }
       rewrite <- hvarsFullShiftEq.
       rewrite MinusHvarShiftEq.
-      assert (ctx_LinOnly (D11 ᴳ+ D12 ᴳ+ D2)) as LinOnlyD. { apply (Ty_ectxs_LinFinOnlyD (D11 ᴳ+ D12 ᴳ+ D2) C (U ⧔ T') U0). tauto. }
+      assert (LinOnly (D11 ᴳ+ D12 ᴳ+ D2)) as LinOnlyD. { apply (Ty_ectxs_LinFinOnlyD (D11 ᴳ+ D12 ᴳ+ D2) C (U ⧔ T') U0). tauto. }
       assert (hvars©( C) ## hvarsᴳ( ᴳ- D13 ᴳ[ hvarsᴳ( ᴳ- D13) ⩲ (maxᴴ( hvars©( C)) + 1)])) as hvarsDisjoint.
-        { rewrite <- MinusHvarShiftEq. rewrite hvarsFullShiftEq. apply hvars_max_hvars_Disjoint with (h' := maxᴴ(hvars©(C)) + 1); rewrite Nat.add_comm; unfold lt, plus; apply le_n_S; reflexivity. }
+        { rewrite <- MinusHvarShiftEq. rewrite hvarsFullShiftEq. apply hvars_max_HDisjoint with (h' := maxᴴ(hvars©(C)) + 1); rewrite Nat.add_comm; unfold lt, plus; apply le_n_S; reflexivity. }
       constructor 19 with (D1 := D2 ᴳ+ D11) (D3 := D13 ᴳ[ hvarsᴳ(ᴳ- D13) ⩲ (maxᴴ(hvars©(C)) + 1)]) (C := C) (v2 := v2 ᵛ[ hvarsᴳ(ᴳ- D13) ⩲ (maxᴴ(hvars©(C)) + 1)]) (T' := T') (U0 := U0) (U := U) (D2 :=
       D12).
         { apply LinOnlyUnionEquiv. rewrite <- UnionAssociative. rewrite UnionCommutative. tauto. }
@@ -2165,20 +2140,20 @@ Proof.
               assert (maxᴴ(hvarsᴳ(D2)) <= maxᴴ(hvars©(C))).
               { apply HmaxSubset. tauto. }
               assert (hvarsᴳ(D2) ## (hvarsᴳ(D13) ᴴ⩲ (maxᴴ(hvars©(C)) + 1))).
-              { apply hvars_max_hvars_Disjoint; rewrite Nat.add_comm; unfold lt, plus; apply le_n_S; tauto. }
+              { apply hvars_max_HDisjoint; rewrite Nat.add_comm; unfold lt, plus; apply le_n_S; tauto. }
               assert (hvarsᴳ(D2) ## hvarsᴳ( D13 ᴳ[ hvarsᴳ(ᴳ- D13) ⩲ (maxᴴ(hvars©(C)) + 1)])).
               { rewrite hvarsMinusEq. rewrite hvarsFullShiftEq. tauto. }
-              apply hvars_DisjointToDisjoint; crush.
+              apply HDisjointToDisjoint; crush.
             }
             { assert (NatSet.Subset hvarsᴳ(D11) hvars©(C)).
               { apply HvarsSubsetCtxUnionBackward in H0. destruct H0. apply HvarsSubsetCtxUnionBackward in H0. tauto. }
               assert (maxᴴ(hvarsᴳ(D11)) <= maxᴴ(hvars©(C))).
               { apply HmaxSubset. tauto. }
               assert (hvarsᴳ(D11) ## (hvarsᴳ(D13) ᴴ⩲ (maxᴴ(hvars©(C)) + 1))).
-              { apply hvars_max_hvars_Disjoint; rewrite Nat.add_comm; unfold lt, plus; apply le_n_S; tauto. }
+              { apply hvars_max_HDisjoint; rewrite Nat.add_comm; unfold lt, plus; apply le_n_S; tauto. }
               assert (hvarsᴳ(D11) ## hvarsᴳ( D13 ᴳ[ hvarsᴳ(ᴳ- D13) ⩲ (maxᴴ(hvars©(C)) + 1)])).
               { rewrite hvarsMinusEq. rewrite hvarsFullShiftEq. tauto. }
-              apply hvars_DisjointToDisjoint; crush.
+              apply HDisjointToDisjoint; crush.
             }
           } } { assert (NatSet.Subset hvarsᴳ(D11 ᴳ+ D12 ᴳ+ D2) hvars©(C)).
               { apply hvars_CWkhvars_G with (U0 := U0) (T := U ⧔ T'). tauto. } 
@@ -2187,10 +2162,10 @@ Proof.
               assert (maxᴴ(hvarsᴳ(D12)) <= maxᴴ(hvars©(C))).
               { apply HmaxSubset. tauto. }
               assert (hvarsᴳ(D12) ## (hvarsᴳ(D13) ᴴ⩲ (maxᴴ(hvars©(C)) + 1))).
-              { apply hvars_max_hvars_Disjoint; rewrite Nat.add_comm; unfold lt, plus; apply le_n_S; tauto. }
+              { apply hvars_max_HDisjoint; rewrite Nat.add_comm; unfold lt, plus; apply le_n_S; tauto. }
               assert (hvarsᴳ(D12) ## hvarsᴳ( D13 ᴳ[ hvarsᴳ(ᴳ- D13) ⩲ (maxᴴ(hvars©(C)) + 1)])).
-              { unfold hvars_Disjoint. rewrite hvarsMinusEq. rewrite hvarsFullShiftEq. tauto. }
-              apply hvars_DisjointToDisjoint. crush. assumption.
+              { unfold HDisjoint. rewrite hvarsMinusEq. rewrite hvarsFullShiftEq. tauto. }
+              apply HDisjointToDisjoint. crush. assumption.
             } } { crush. } { crush. } { crush. } { crush. } { crush. } { crush. } { rewrite UnionCommutative in TyC. rewrite UnionAssociative in TyC. tauto. }
           { rewrite <- D12Eq. rewrite <- MinusHvarShiftEq. rewrite <- UnionHvarShiftEq. apply TyR_v_hvar_shift. tauto.  } { assumption. }
     - (* Sem-eterm-AOpenUnfoc *)
@@ -2201,9 +2176,9 @@ Proof.
         { unfold ctx_union, merge_with, merge. apply ext_eq. intros n. all:simpl. rewrite H0. reflexivity. }
       rewrite <- eqD1uD3PuD in *. clear H0. clear eqD1uD3PuD. clear D.
       assert (D1 ᴳ+ D2 ⊢ ᵥ₎ hvarsᴳ(ᴳ- D3) ⟨ v2 ❟ v1 ⟩ : U ⧔ T) as TyA.
-        { term_Val_no_dispose (D1 ᴳ+ D2). apply Ty_ectxs_hvars_Disjoint with (D := D1 ᴳ+ D2) (D' := (ᴳ- D3)) (C := C) (T := U ⧔ T) (U0 := U0) in hvarsDisjoint. apply TyR_val_A. all: trivial. crush.
+        { term_Val_no_dispose (D1 ᴳ+ D2). apply Ty_ectxs_HDisjoint with (D := D1 ᴳ+ D2) (D' := (ᴳ- D3)) (C := C) (T := U ⧔ T) (U0 := U0) in hvarsDisjoint. apply TyR_val_A. all: trivial. crush.
          }
-      assert (ctx_LinOnly (D1 ᴳ+ D2)) as LinOnlyD.
+      assert (LinOnly (D1 ᴳ+ D2)) as LinOnlyD.
         { apply (Ty_ectxs_LinFinOnlyD (D1 ᴳ+ D2) C (U ⧔ T) U0). tauto. }
       constructor 1 with (D := (D1 ᴳ+ D2)) (T := U ⧔ T) (t := ᵥ₎ hvarsᴳ(ᴳ- D3) ⟨ v2 ❟ v1 ⟩). all: crush.
 (*     - (* Sem-eterm-AllocRed *)
@@ -2236,14 +2211,14 @@ Proof.
     - (* Sem-eterm-ToAFoc *)
       inversion Tyt; subst.
       rename Tyt into TyToA.
-      assert (ctx_LinOnly D) as LinOnlyD.
+      assert (LinOnly D) as LinOnlyD.
         { apply (Ty_ectxs_LinFinOnlyD D C (U ⧔ ①) U0). tauto. }
       constructor 1 with (D := D) (t := u) (T := U); swap 1 3. constructor 9. all: crush.
     - (* Sem-eterm-ToAUnfoc *)
       inversion Tyt; subst. rename TyC into TyCc, T into U. clear H1.
       inversion TyCc; subst. rename D0 into D.
       rewrite (SimplifyDisposableInTyC P D DisposP DestOnlyD) in *.
-      assert (ctx_LinOnly D) as LinOnlyD.
+      assert (LinOnly D) as LinOnlyD.
         { apply (Ty_ectxs_LinFinOnlyD D C (U ⧔ ①) U0). tauto. }
       assert (D ⊢ to⧔ ᵥ₎ v2 : U ⧔ ①) as TyToA.
         { apply (Ty_term_ToA D (ᵥ₎ v2) U). tauto. }
@@ -2263,14 +2238,14 @@ Proof.
     - (* Sem-eterm-FromAFoc *)
       inversion Tyt; subst.
       rename Tyt into TyFromA, T into U.
-      assert (ctx_LinOnly D) as LinOnlyD.
+      assert (LinOnly D) as LinOnlyD.
         { apply (Ty_ectxs_LinFinOnlyD D C U U0). tauto. }
       constructor 1 with (D := D) (t := t) (T := U ⧔ ①); swap 1 3. constructor 10. all: crush.
     - (* Sem-eterm-FromAUnfoc *)
       inversion Tyt; subst. rename TyC into TyCc, T into U, D0 into D. clear H1.
       inversion TyCc; subst. rename U1 into U, v into v2, D into D2, ValidOnlyD into ValidOnlyD2, DestOnlyD into DestOnlyD2.
       rewrite (SimplifyDisposableInTyC P D2 DisposP DestOnlyD2) in *.
-      assert (ctx_LinOnly D2) as LinOnlyD2.
+      assert (LinOnly D2) as LinOnlyD2.
         { apply (Ty_ectxs_LinFinOnlyD D2 C U U0). tauto. }
       assert (D2 ⊢ from⧔ ᵥ₎ v2 : U) as TyFromA.
         { apply (Ty_term_FromA D2 (ᵥ₎ v2) U). tauto. }
@@ -2293,14 +2268,14 @@ Proof.
     - (* Sem-eterm-FillUFoc *)
       inversion Tyt; subst.
       rename Tyt into TyFillU, Tyt0 into Tyt.
-      assert (ctx_LinOnly D) as LinOnlyD.
+      assert (LinOnly D) as LinOnlyD.
         { apply (Ty_ectxs_LinFinOnlyD D C ① U0). tauto. }
       constructor 1 with (D := D) (t := t) (T := ⌊ ① ⌋ n); swap 1 3. constructor 11. all: crush.
     - (* Sem-eterm-FillUUnfoc *)
       inversion Tyt; subst. rename TyC into TyCc, T into U. clear H1.
       inversion TyCc; subst. rename D0 into D.
       rewrite (SimplifyDisposableInTyC P D DisposP DestOnlyD) in *.
-      assert (ctx_LinOnly D) as LinOnlyD.
+      assert (LinOnly D) as LinOnlyD.
         { apply (Ty_ectxs_LinFinOnlyD D C ① U0). tauto. }
       assert (D ⊢ ᵥ₎ v⨞() : ①) as TyFillU.
         { apply (Ty_term_FillU D (ᵥ₎ v) n). tauto. }
@@ -2308,7 +2283,7 @@ Proof.
     - (* Sem-eterm-FillURed *)
       inversion Tyt; subst.
       rename Tyt into TyFillU, Tyt0 into Tytp.
-      assert (ctx_LinOnly D /\ ctx_FinAgeOnly D) as (LinOnlyD & FinAgeOnlyD).
+      assert (LinOnly D /\ FinAgeOnly D) as (LinOnlyD & FinAgeOnlyD).
         { apply (Ty_ectxs_LinFinOnlyD D C ① U0). tauto. }
       inversion Tytp; subst. clear H1.
       inversion TyRv; subst.
@@ -2328,14 +2303,14 @@ Proof.
     - (* Sem-eterm-FillLFoc *)
       inversion Tyt; subst.
       rename Tyt into TyFillL, Tyt0 into Tyt.
-      assert (ctx_LinOnly D) as LinOnlyD.
+      assert (LinOnly D) as LinOnlyD.
         { apply (Ty_ectxs_LinFinOnlyD D C (⌊ T1 ⌋ n) U0). tauto. }
       constructor 1 with (D := D) (t := t) (T := ⌊ T1 ⨁ T2 ⌋ n); swap 1 3. constructor 12. all: crush.
     - (* Sem-eterm-FillLUnfoc *)
       inversion Tyt; subst. rename TyC into TyCc, T into U. clear H1.
       inversion TyCc; subst. rename D0 into D.
       rewrite (SimplifyDisposableInTyC P D DisposP DestOnlyD) in *.
-      assert (ctx_LinOnly D) as LinOnlyD.
+      assert (LinOnly D) as LinOnlyD.
         { apply (Ty_ectxs_LinFinOnlyD D C (⌊ T1 ⌋ n) U0). tauto. }
       assert (D ⊢ ᵥ₎ v ⨞Inl : ⌊ T1 ⌋ n) as TyFillL.
         { apply (Ty_term_FillL D (ᵥ₎ v) T1 n T2). tauto. }
@@ -2343,7 +2318,7 @@ Proof.
     - (* Sem-eterm-FillLRed *)
       inversion Tyt; revert hpMaxCh; subst.
       rename Tyt into TyFillL, Tyt0 into Tytp.
-      assert (ctx_LinOnly D /\ ctx_FinAgeOnly D) as (LinOnlyD & FinAgeOnlyD).
+      assert (LinOnly D /\ FinAgeOnly D) as (LinOnlyD & FinAgeOnlyD).
         { apply (Ty_ectxs_LinFinOnlyD D C (⌊ T1 ⌋ n) U0). tauto. }
       inversion Tytp; subst. clear H1. rename D0 into D.
       rewrite (SimplifyDisposableInTyC P D DisposP DestOnlyD) in *.
@@ -2385,74 +2360,74 @@ Proof.
   - rename v into v', v0 into v, D into D2, ValidOnlyD into ValidOnlyD2. clear DestOnlyD. exists C, (ᵥ₎ v ⨞· ᵥ₎ v'). constructor.
   - rename v into v1, TyRv into TyRv1. exists C, (ᵥ₎ hvarsᴳ(ᴳ- D3) ⟨ v2 ❟ v1 ⟩). constructor.
   - assert (P ᴳ+ ᴳ{ x : m ‗ T} = ᴳ{ x : m ‗ T}) as elimP. { apply SimplifyDisposableInTyC; tauto. } rewrite elimP in *.
-    exfalso. unfold ctx_DestOnly in DestOnlyD. specialize (DestOnlyD (ˣ x) (ₓ m ‗ T)). unfold ctx_singleton in DestOnlyD. rewrite singleton_MapsKeyTo in DestOnlyD. specialize (DestOnlyD eq_refl). unfold binding_IsDest in DestOnlyD. contradiction.
+    exfalso. unfold DestOnly in DestOnlyD. specialize (DestOnlyD (ˣ x) (ₓ m ‗ T)). unfold ctx_singleton in DestOnlyD. rewrite singleton_MapsKeyTo in DestOnlyD. specialize (DestOnlyD eq_refl). unfold IsDest in DestOnlyD. contradiction.
   - rename Tyt into TyApp, T into U, T0 into T, t0 into t, Tyt0 into Tyt, P1 into D1, P2 into D2.
-    destruct (term_NotVal_dec t). all: try destruct e; subst. all: try rename x into v.
-    * destruct (term_NotVal_dec t'). all: try destruct e; subst. all: try rename x into v'.
+    destruct (NotVal_dec t). all: try destruct e; subst. all: try rename x into v.
+    * destruct (NotVal_dec t'). all: try destruct e; subst. all: try rename x into v'.
       + inversion Tytp; subst. inversion TyRv; subst. { exfalso. apply TyR_val_DestOnlyValHole with (D := ᴳ{- h : T ⁔ m → U ‗ ¹ν}) (h := h) (T := T ⁔ m → U); tauto. }
       exists C, (u ᵗ[x ≔ v]). constructor.
       + exists (C ∘ (v ≻⬜)), t'. constructor; tauto.
     * exists (C ∘ ⬜≻ t'), t. constructor; tauto.
-  - rename Tyt into TyPatU, T into U, t0 into t, Tyt0 into Tyt, P1 into D1, P2 into D2. destruct (term_NotVal_dec t).
+  - rename Tyt into TyPatU, T into U, t0 into t, Tyt0 into Tyt, P1 into D1, P2 into D2. destruct (NotVal_dec t).
     * destruct e; subst. rename x into v. inversion Tyt; subst. inversion TyRv; subst. { exfalso. apply TyR_val_DestOnlyValHole with (D := ᴳ{- h : ① ‗ ¹ν}) (h := h) (T := ①); tauto. } exists C, u. constructor.
     * exists (C ∘ ⬜; u), t. constructor; tauto.
-  - rename Tyt into TyPatS, T into U, t0 into t, Tyt0 into Tyt, P1 into D1, P2 into D2. destruct (term_NotVal_dec t).
+  - rename Tyt into TyPatS, T into U, t0 into t, Tyt0 into Tyt, P1 into D1, P2 into D2. destruct (NotVal_dec t).
     * destruct e; subst. rename x into v. inversion Tyt; subst. inversion TyRv; subst. { exfalso. apply TyR_val_DestOnlyValHole with (D := ᴳ{- h : T1 ⨁ T2 ‗ ¹ν}) (h := h) (T := T1 ⨁ T2); tauto. }
       { exists C, (u1 ᵗ[x1 ≔ v1]). constructor. }
       { exists C, (u2 ᵗ[x2 ≔ v2]). constructor. }
     * exists (C ∘ (⬜≻caseˢ m {Inl x1 ⟼ u1, Inr x2 ⟼ u2})), t. constructor; tauto.
-  - rename Tyt into TyPatP, T into U, t0 into t, Tyt0 into Tyt, P1 into D1, P2 into D2. destruct (term_NotVal_dec t).
+  - rename Tyt into TyPatP, T into U, t0 into t, Tyt0 into Tyt, P1 into D1, P2 into D2. destruct (NotVal_dec t).
     * destruct e; subst. rename x into v. inversion Tyt; subst. inversion TyRv; subst. { exfalso. apply TyR_val_DestOnlyValHole with (D := ᴳ{- h : T1 ⨂ T2 ‗ ¹ν}) (h := h) (T := T1 ⨂ T2); tauto. }
       { exists C, (u ᵗ[x1 ≔ v1] ᵗ[x2 ≔ v2]). constructor. }
     * exists (C ∘ ⬜≻caseᵖ m ᵗ( x1, x2)⟼ u), t. constructor; tauto.
-  - rename Tyt into TyPatE, T into U, T0 into T, t0 into t, Tyt0 into Tyt, P1 into D1, P2 into D2. destruct (term_NotVal_dec t).
+  - rename Tyt into TyPatE, T into U, T0 into T, t0 into t, Tyt0 into Tyt, P1 into D1, P2 into D2. destruct (NotVal_dec t).
     * destruct e; subst. rename x0 into v. inversion Tyt; subst. inversion TyRv; subst. { exfalso. apply TyR_val_DestOnlyValHole with (D := ᴳ{- h : ! n ⁔ T ‗ ¹ν}) (h := h) (T := ! n ⁔ T); tauto. }
       { exists C, (u ᵗ[x ≔ v']). constructor. }
     * exists (C ∘ ⬜≻caseᵉ m ᴇ n ⁔ x ⟼ u), t. constructor; tauto.
-  - rename Tyt into TyMap, t0 into t, Tyt0 into Tyt, P1 into D1, P2 into D2. destruct (term_NotVal_dec t).
+  - rename Tyt into TyMap, t0 into t, Tyt0 into Tyt, P1 into D1, P2 into D2. destruct (NotVal_dec t).
     * destruct e; subst. rename x0 into v. inversion Tyt; subst. inversion TyRv; subst. { exfalso. apply TyR_val_DestOnlyValHole with (D := ᴳ{- h : U ⧔ T ‗ ¹ν}) (h := h) (T := U ⧔ T); tauto. }
-      rename D2 into D', D0 into D2. assert (ctx_DestOnly (P ᴳ+ (D1 ᴳ+ D2))) as DestOnlyPuD1uD2. { crush. } rewrite (SimplifyDisposableInTyC P (D1 ᴳ+ D2) DisposP DestOnlyPuD1uD2) in *.
+      rename D2 into D', D0 into D2. assert (DestOnly (P ᴳ+ (D1 ᴳ+ D2))) as DestOnlyPuD1uD2. { crush. } rewrite (SimplifyDisposableInTyC P (D1 ᴳ+ D2) DisposP DestOnlyPuD1uD2) in *.
       exists (C ∘ hvarsᴳ(ᴳ- D3) ᴴ⩲ (maxᴴ(hvars©(C)) + 1) ᵒᵖ⟨ v2 ᵛ[hvarsᴳ(ᴳ- D3) ⩲ (maxᴴ(hvars©(C)) + 1)] ❟⬜), (t' ᵗ[x ≔ v1 ᵛ[hvarsᴳ(ᴳ- D3) ⩲ (maxᴴ(hvars©(C)) + 1)]]). constructor; tauto.
     * exists (C ∘ ⬜≻map x ⟼ t'), t. constructor; tauto.
-  - rename Tyt into TyToA. destruct (term_NotVal_dec u).
+  - rename Tyt into TyToA. destruct (NotVal_dec u).
     * destruct e; subst. rename x into v2. exists C, (ᵥ₎ NatSet.empty ⟨ v2 ❟ ᵛ() ⟩ ). constructor.
     * exists (C ∘ to⧔⬜), u. constructor; tauto.
-  - rename Tyt into TyToA, Tyt0 into Tyt, t0 into t. destruct (term_NotVal_dec t).
+  - rename Tyt into TyToA, Tyt0 into Tyt, t0 into t. destruct (NotVal_dec t).
     * destruct e; subst. rename x into v. inversion Tyt; subst. inversion TyRv; subst. { exfalso. apply TyR_val_DestOnlyValHole with (D := ᴳ{- h : T ⧔ ① ‗ ¹ν}) (h := h) (T := T ⧔ ①); tauto. }
-      inversion TyRv1; subst. { assert (ctx_DestOnly (¹↑ ᴳ· D1 ᴳ+ D3)). { crush. } exfalso. apply TyR_val_DestOnlyValHole with (D := (¹↑ ᴳ· D1 ᴳ+ D3)) (h := h) (T := ①). all:tauto. }
+      inversion TyRv1; subst. { assert (DestOnly (¹↑ ᴳ· D1 ᴳ+ D3)). { crush. } exfalso. apply TyR_val_DestOnlyValHole with (D := (¹↑ ᴳ· D1 ᴳ+ D3)) (h := h) (T := ①). all:tauto. }
       assert (¹↑ ᴳ· D1 ᴳ+ D3 = ᴳ{}) as Empty.
       { apply ext_eq'. symmetry. apply H0. }
       apply empty_union in Empty. destruct Empty as [_ EmptyD3].
       subst. rewrite hvarsMinusEq, hvarsEmpty.
       exists C, (ᵥ₎ v2). constructor.
     * exists (C ∘ from⧔⬜), t. constructor; tauto.
-  - rename Tyt into TyFillU, Tyt0 into Tyt, t0 into t. destruct (term_NotVal_dec t).
+  - rename Tyt into TyFillU, Tyt0 into Tyt, t0 into t. destruct (NotVal_dec t).
     * destruct e; subst. rename x into v. inversion Tyt; subst. inversion TyRv; subst. { exfalso. apply TyR_val_DestOnlyValHole with (D := ᴳ{- h : ⌊ ① ⌋ n ‗ ¹ν}) (h := h) (T := ⌊ ① ⌋ n); tauto. }
       exists (C ©️[ h ≔ NatSet.empty ‗ ᵛ()]), (ᵥ₎ ᵛ()). constructor.
     * exists (C ∘ ⬜⨞()), t. constructor; tauto.
-  - rename Tyt into TyFillL, Tyt0 into Tyt, t0 into t. destruct (term_NotVal_dec t).
+  - rename Tyt into TyFillL, Tyt0 into Tyt, t0 into t. destruct (NotVal_dec t).
     * destruct e; subst. rename x into v. inversion Tyt; subst. inversion TyRv; subst. { exfalso. apply TyR_val_DestOnlyValHole with (D := ᴳ{- h : ⌊ T1 ⨁ T2 ⌋ n ‗ ¹ν}) (h := h) (T := ⌊ T1 ⨁ T2 ⌋ n); tauto. }
     exists (C ©️[ h ≔ ᴴ{ maxᴴ( hvars©(C) ∪ ᴴ{ h}) + 1 + 1} ‗ Inl ᵛ- (maxᴴ( hvars©(C) ∪ ᴴ{ h}) + 1 + 1)]), (ᵥ₎ ᵛ+ (maxᴴ( hvars©(C) ∪ ᴴ{ h}) + 1 + 1)). constructor; tauto.
     * exists (C ∘ ⬜⨞Inl), t. constructor; tauto.
-  - rename Tyt into TyFillR, Tyt0 into Tyt, t0 into t. destruct (term_NotVal_dec t).
+  - rename Tyt into TyFillR, Tyt0 into Tyt, t0 into t. destruct (NotVal_dec t).
     * destruct e; subst. rename x into v. inversion Tyt; subst. inversion TyRv; subst. { exfalso. apply TyR_val_DestOnlyValHole with (D := ᴳ{- h : ⌊ T1 ⨁ T2 ⌋ n ‗ ¹ν}) (h := h) (T := ⌊ T1 ⨁ T2 ⌋ n); tauto. }
     exists (C ©️[ h ≔ ᴴ{ maxᴴ( hvars©(C) ∪ ᴴ{ h}) + 1 + 1} ‗ Inr ᵛ- (maxᴴ( hvars©(C) ∪ ᴴ{ h}) + 1 + 1)]), (ᵥ₎ ᵛ+ (maxᴴ( hvars©(C) ∪ ᴴ{ h}) + 1 + 1)). constructor; tauto.
     * exists (C ∘ ⬜⨞Inr), t. constructor; tauto.
-  - rename Tyt into TyFillP, Tyt0 into Tyt, t0 into t. destruct (term_NotVal_dec t).
+  - rename Tyt into TyFillP, Tyt0 into Tyt, t0 into t. destruct (NotVal_dec t).
     * destruct e; subst. rename x into v. inversion Tyt; subst. inversion TyRv; subst. { exfalso. apply TyR_val_DestOnlyValHole with (D := ᴳ{- h : ⌊ T1 ⨂ T2 ⌋ n ‗ ¹ν}) (h := h) (T := ⌊ T1 ⨂ T2 ⌋ n); tauto. }
     exists (C ©️[ h ≔ ᴴ{ maxᴴ( hvars©(C) ∪ ᴴ{ h}) + 1 + 1 , maxᴴ( hvars©(C) ∪ ᴴ{ h}) + 1 + 2} ‗ ᵛ( ᵛ- (maxᴴ( hvars©(C) ∪ ᴴ{ h}) + 1 + 1), ᵛ- (maxᴴ( hvars©(C) ∪ ᴴ{ h}) + 1 + 2))]), (ᵥ₎ ᵛ( ᵛ+ (maxᴴ( hvars©(C) ∪ ᴴ{ h}) + 1 + 1), ᵛ+ (maxᴴ( hvars©(C) ∪ ᴴ{ h}) + 1 + 2))). constructor; tauto.
     * exists (C ∘ ⬜⨞(,)), t. constructor; tauto.
-  - rename Tyt into TyFillE, Tyt0 into Tyt, t0 into t. destruct (term_NotVal_dec t).
+  - rename Tyt into TyFillE, Tyt0 into Tyt, t0 into t. destruct (NotVal_dec t).
     * destruct e; subst. rename x into v. inversion Tyt; subst. inversion TyRv; subst. { exfalso. apply TyR_val_DestOnlyValHole with (D := ᴳ{- h : ⌊ ! n' ⁔ T ⌋ n ‗ ¹ν}) (h := h) (T := ⌊ ! n' ⁔ T ⌋ n); tauto. }
     exists (C ©️[ h ≔ ᴴ{ maxᴴ( hvars©(C) ∪ ᴴ{ h}) + 1 + 1} ‗ ᴇ n' ⁔ ᵛ- (maxᴴ( hvars©(C) ∪ ᴴ{ h}) + 1 + 1)]), (ᵥ₎ ᵛ+ (maxᴴ( hvars©(C) ∪ ᴴ{ h}) + 1 + 1)). constructor; tauto.
     * exists (C ∘ ⬜⨞ᴇ n'), t. constructor; tauto.
-  - rename Tyt into TyFillF, Tyt0 into Tyt, t0 into t. destruct (term_NotVal_dec t).
+  - rename Tyt into TyFillF, Tyt0 into Tyt, t0 into t. destruct (NotVal_dec t).
     * destruct e; subst. rename x0 into v. inversion Tyt; subst. inversion TyRv; subst. { exfalso. apply TyR_val_DestOnlyValHole with (D := ᴳ{- h : ⌊ T ⁔ m → U ⌋ n ‗ ¹ν}) (h := h) (T := ⌊ T ⁔ m → U ⌋ n); tauto. }
     exists (C ©️[ h ≔ NatSet.empty ‗ λᵛ x ⁔ m ⟼ u ]), (ᵥ₎ ᵛ()). constructor; tauto.
     * exists (C ∘ ⬜⨞(λ x ⁔ m ⟼ u)), t. constructor; tauto.
-  - rename Tyt into TyFillC, Tyt0 into Tyt, t0 into t, P1 into D1, P2 into D2. destruct (term_NotVal_dec t).
-    * destruct e; subst. rename x into v. destruct (term_NotVal_dec t').
-      + destruct e; subst. rename x into v'. inversion Tyt; subst. inversion TyRv; subst. { exfalso. apply TyR_val_DestOnlyValHole with (D := ᴳ{- h : ⌊ U ⌋ n ‗ ¹ν}) (h := h) (T := ⌊ U ⌋ n); tauto. } rename H1 into DestOnlyD'. inversion Tytp; subst. rename TyRv0 into TyRvp. inversion TyRvp; subst. { exfalso. apply TyR_val_DestOnlyValHole with (D := ᴳ{- h0 : U ⧔ T ‗ ¹ν}) (h := h0) (T := U ⧔ T); tauto. } assert (ctx_DestOnly (P0 ᴳ+ (D1 ᴳ+ D2))) as DestOnlyP0uD1uD2. { crush. } rewrite (SimplifyDisposableInTyC P0 (D1 ᴳ+ D2) DisposP0 DestOnlyP0uD1uD2) in *.
+  - rename Tyt into TyFillC, Tyt0 into Tyt, t0 into t, P1 into D1, P2 into D2. destruct (NotVal_dec t).
+    * destruct e; subst. rename x into v. destruct (NotVal_dec t').
+      + destruct e; subst. rename x into v'. inversion Tyt; subst. inversion TyRv; subst. { exfalso. apply TyR_val_DestOnlyValHole with (D := ᴳ{- h : ⌊ U ⌋ n ‗ ¹ν}) (h := h) (T := ⌊ U ⌋ n); tauto. } rename H1 into DestOnlyD'. inversion Tytp; subst. rename TyRv0 into TyRvp. inversion TyRvp; subst. { exfalso. apply TyR_val_DestOnlyValHole with (D := ᴳ{- h0 : U ⧔ T ‗ ¹ν}) (h := h0) (T := U ⧔ T); tauto. } assert (DestOnly (P0 ᴳ+ (D1 ᴳ+ D2))) as DestOnlyP0uD1uD2. { crush. } rewrite (SimplifyDisposableInTyC P0 (D1 ᴳ+ D2) DisposP0 DestOnlyP0uD1uD2) in *.
       exists
         ( C ©️[ h ≔ hvarsᴳ(ᴳ- D3) ᴴ⩲ (maxᴴ( hvars©(C) ∪ ᴴ{ h}) + 1) ‗  v2 ᵛ[hvarsᴳ(ᴳ- D3) ⩲ (maxᴴ( hvars©(C) ∪ ᴴ{ h}) + 1)] ] ),
         (ᵥ₎ v1 ᵛ[hvarsᴳ(ᴳ- D3) ⩲ (maxᴴ( hvars©(C) ∪ ᴴ{ h}) + 1)]).
